remove old PathORAM.v and rename PathORAM_typeclasses.v to PathORAM.v

theory/System/PathORAM.v
@@ -1,1152 +1,2813 @@
-Require Import List.
+Require Coq.Bool.Bool.
+Require Import Coq.Vectors.Vector.
+Require Import Coq.Lists.List.
+Require Import Coq.QArith.QArith.
+Require Import Coq.Classes.EquivDec.
 Import ListNotations.
-From Coq Require Import Lia.
-Require Import Coq.Bool.Bool.
-Require Import Coq.Arith.EqNat.
-Require Import Coq.Arith.Even.
-Require Import Coq.Init.Datatypes.
-Require Import Coq.Strings.String.
-Require Import Coq.NArith.BinNat. 
-Require Import Coq.Program.Wf.
-Require Import Streams.
-Require Import Coq.ZArith.Zdiv.
-
-
-Require Import  ExtLib.Data.Monads.StateMonad ExtLib.Structures.Monads.
-Search Monad.
-Import MonadLetNotation.
-Open Scope monad_scope.
-
-Section Utils.
-
-End Utils.
-
-Section Tree.
-(* (***************************************) *)
-(* (*************** STASH *****************) *)
-(* (***************************************) *)
-
-
-(* Section STASH. *)
-  Definition concatStash {A} (stsh : list (prod nat A)) (a : list (prod nat A)) := stsh ++ a.
-
-  Inductive BlockEntry : Type := BV(f s: nat).
-
-  Definition BlockEntry_fst (be : BlockEntry) : nat :=
-    match be with
-    | BV f _ => f
-    end.
-      
-  Fixpoint readBlockFromStash (stsh : list BlockEntry) (bID : nat) : option nat :=
-    match stsh with
-    | [] => None
-    | h :: t => match h with
-              | BV f s => if Nat.eqb f bID
-                        then Some s
-                        else readBlockFromStash t bID
-              end
-                
-    end.
-  
-  
-  Fixpoint updateStash(bID: nat) (dataN: nat)(stsh: list BlockEntry): list BlockEntry :=
-    match stsh with
-    | [] => []
-    | (BV id data) :: t => if Nat.eqb bID id
-                       then (BV id dataN) :: updateStash bID dataN t
-                       else updateStash bID dataN t
-    end.
-      
-  Fixpoint popStash (stsh: list BlockEntry) (sublist: list BlockEntry) : list BlockEntry :=
-    match sublist with
-    | [] => stsh
-    | (BV k v) :: t =>
-        match stsh with
-        | [] => []
-        | (BV bID data) :: xs =>
-            if Nat.eqb k bID
-            then xs
-            else popStash stsh t
-        end
-    end.
-
-  Fixpoint popList {A} (a s : list A) (f : A -> A -> bool): list A :=
-    match s with
-    | [] => a
-    | h :: t => match a with
-              | [] => []
-              | x :: xs => if f h x
-                         then popList xs t f 
-                         else popList xs s f 
-              end
-    end.
-      
-(* Compute popList [1;2;3;4;5] [1;5;2] Nat.eqb. PROBLEMATIC.*)
-  
-(* End STASH. *)
-
-
-
-  
-  Inductive PBTree (A: Type) : Type :=
-  | Leaf (idx: nat) (val: A)
-  | Node (idx: nat) (val: A) (l r: PBTree A).
-
-
-  (* Fixpoint RBTree (A: Type) (l : nat): Type := *)
-  (*   match l with *)
-  (*     | O =>  *)
-  
-
-  Fixpoint pb (X : Type) (n : nat) : Type :=
-    match n with
-    | 0 => unit
-    | S m => X * pb X m * pb X m
-    end.
-
-  Definition leaf {X} : pb X 0 := tt.
-
-  Definition node {X} {n} : X -> pb X n -> pb X n -> pb X (S n) :=
-    fun x t1 t2 => (x,t1,t2).
-
-  Definition example : pb nat 2 :=
-    node 0
-         (node 1 leaf leaf)
-         (node 2 leaf leaf).
-
-
-  Arguments Leaf {_} _ _.
-  Arguments Node {_} _ _ _ _.
-
-  Fixpoint getHeight {A: Type} (root: PBTree A) : nat :=
-    match root with
-    | Leaf _ _ => 0
-    | Node _ _ l r => S (max (getHeight l) (getHeight r))
-    end.
-
-
-  Fixpoint isPBTree {A} (t : PBTree A) : Prop :=
-    match t with
-    | Leaf _ _ => True
-    | Node _ _ l r => getHeight l = getHeight r
-                     /\ (isPBTree l) /\( isPBTree r)
-    end.
-  
-                       
-  Fixpoint buildPBTlevelOrder {A} (def_a : A) (label : nat) (ht : nat) : PBTree A :=
-    match ht with
-    | 0 => Leaf label def_a
-    | S ht' => Node label def_a
-                      (buildPBTlevelOrder def_a (2 * label + 1) ht')
-                      (buildPBTlevelOrder def_a (2 * label + 2) ht')
-    end.
-  
-  Definition PBTree1 {A} : PBTree (list A) := buildPBTlevelOrder [] 0 3.
-
-  Compute PBTree1.
-  
-  Inductive Dir := L | R.
-
-  Lemma div2 : forall (n : nat), PeanoNat.Nat.div2 n  < S n.
-  Proof.
-    fix IH 1.
-    intro n. case n.
-    - constructor.
-    - intro n0. case n0.
-      + constructor. constructor.
-      + intro n1. specialize (IH n1). simpl.
-        apply Lt.lt_n_S.
-        apply PeanoNat.Nat.lt_lt_succ_r. apply IH.
-  Defined.
-
-  Program Fixpoint getPath (lfIdx : nat) {measure lfIdx} : list Dir :=
-    match lfIdx with
-    | 0 => []
-    | S idx => if Nat.even idx
-              then [L] ++ getPath (PeanoNat.Nat.div2 idx)
-              else [R] ++ getPath (PeanoNat.Nat.div2 idx)
-    end.
-  Next Obligation.
-    apply div2.
-    Qed.
-  Next Obligation.
-  apply div2.
-  Defined.
-
-  Compute getPath 8.
-  Definition p9 := getPath 9.
-
-  Compute getPath 12.
-  Definition p12 := getPath 12.
-
-  Fixpoint buildNodeLevelDict {A} (root: PBTree A) (currL : nat) : list (prod nat nat) :=
-    match root with
-    | Leaf idx val => [pair idx currL]
-    | Node idx val l r =>
-        [pair idx currL] ++ buildNodeLevelDict l (S currL)  ++ buildNodeLevelDict r (S currL)
-    end.
-
-  Compute buildNodeLevelDict PBTree1 0.
-
-  Fixpoint writeAtPath {A} (root : PBTree A)
-           (path : list Dir) (data : A) : PBTree A :=
-    match root with
-    | Leaf idx val =>
-        match path with
-        | [] => Leaf idx data
-        | _ => Leaf idx val (* path longer than height of tree*)
-        end
-    | Node idx val l r =>
-        match path with
-        | [] => Node idx data l r
-        | L :: path' => Node idx val (writeAtPath l path' data) r
-        | R :: path' => Node idx val l (writeAtPath r path' data)
-        end
-    end.
-
-
-
-  Compute writeAtPath PBTree1 p12 [1;2;3].
-  Compute writeAtPath PBTree1 p9 [4;5;6].
-  Compute writeAtPath PBTree1 (getPath 4) [5;5;5]. (* 4 and 5 seem to be flipped *)
-  
-  Definition writeToNode {A} (root : PBTree A) (lfIdx : nat) (tgtl : nat) (data : A) : PBTree A :=
-    writeAtPath root (firstn tgtl (getPath lfIdx)) data. 
-
-  Compute PBTree1.
-  Compute writeToNode PBTree1 9 2 [0; 1; 2].
-  
-  (* Definition of rand comes from Yves Bertot *)
-  CoFixpoint rand (seed n1 n2 : Z) : Stream Z :=
-    let seed' := Zmod seed n2 in Cons seed' (rand (seed' * n1) n1 n2).           
-  (* find a definition of one-way function with unique inputs *)
-  
-  Fixpoint takeS {X} n (str : Stream X) : list X :=
-    match n with
-    | 0 => []
-    | S m => match str with
-            | Cons x str' => x :: takeS m str'
-            end
-    end.
-
-  Compute  takeS 60(rand 475 919 953).
-  Definition first60 := takeS 60(rand 475 919 953).
-
-  Definition md_tot := fun x => Zmod x 15.
-
-  Compute List.map Z.to_nat (List.map md_tot first60).
-  Definition randSeq := List.map Z.to_nat (List.map md_tot first60).
-
-  Fixpoint modNodesTotal (randList : list Z) : list nat :=
-    List.map Z.to_nat(List.map md_tot randList).
-
-  Fixpoint indexed_list {X} (start : nat) (l : list X) : list (nat * X) :=
-    match l with
-    | [] => []
-    | h :: t => (start, h) :: indexed_list (S start) t
-    end.
-
-  Compute indexed_list 0 randSeq.
-  Definition position_map := indexed_list 0 randSeq.
-
-  Fixpoint posMpLookUp {X} (psmp: list (nat * X)) (id: nat) : option X :=
-    match psmp with
-    | [] => None
-    | (k, v) :: t => if Nat.eqb k id
-                   then Some v
-                   else posMpLookUp t id
-    end.
-      
-      
-  Fixpoint aggregation_helper (key : nat)(val : nat)(l : list (nat * (list nat))):
-    list (nat * (list nat)) :=
-    match l with
-    | [] => [(key, [val])]
-    | (n, al) :: t => if Nat.eqb n key
-                  then (key, val :: al) :: t 
-                  else (n, al) :: aggregation_helper key val t
-    end.
-           
-  Fixpoint aggregation (l : list (nat * nat)): list (nat * (list nat)):=
-    match l with
-    | [] =>  []
-    | (b, n) :: t => aggregation_helper n b (aggregation t)
-    end.
-
-  Compute aggregation [(1, 3); (2,3); (8, 3); (4, 4); (5,4)].
-  Definition n_bl_pair := aggregation [(1, 3); (2,3); (8, 3); (4, 4); (5,4)].
-
-  Fixpoint makeNZeros (n : nat) : list nat :=
-    match n with
-    | O => []
-    | S n' => O :: makeNZeros n'
-    end.
-
-  Compute makeNZeros 10.
-
-
-  Fixpoint takeL {A} n (l : list A) : list A :=
-    match n with
-    | O => []
-    | S m => match l with
-            | [] => []
-            | h :: t => h :: takeL m t 
-            end
-    end.
-
-  Compute takeL 4 [1;2;3].
-  
-  Fixpoint takeFromIdx {A} (n : nat) (l : list A)  : list A :=
-    match l with
-    | [] => []
-    | h :: t => match n with
-              | O => h :: t
-              | S m => takeFromIdx m t
-              end
-    end.
-
-  Compute takeFromIdx 2 [1; 2; 3;4].
-  
-  
-  Fixpoint pairGen {A} (l : list(nat * list nat)) (rt : PBTree A ): list (nat * nat) :=
-    match l with
-    | [] => []
-    | (n, bs) :: t => match rt with
-                    | Leaf idx _ => if Nat.eqb n idx
-                                   then List.combine bs (makeNZeros (List.length bs))
-                                                     (* expand this n's bs *)
-                                   else pairGen t rt (* recurse  *)
-                    | Node idx _ l r => if Nat.eqb n idx
-                                       then List.combine bs (makeNZeros (List.length bs))
-                                                         (* expand this n's bs *)
-                                       else pairGen t rt  (* recurse  *)
-                    end
-    end.
-
-  Compute pairGen n_bl_pair (Leaf 3 3).
-  Compute takeL 2 (pairGen n_bl_pair (Leaf 3 3)). 
-
-  Check writeAtPath.
-
-  Definition initialT A := (PBTree A, list(nat * nat)).
-
-  Print option.
-
-  (* define type of the initialzation function; needs to talk to Big T*)
-  Inductive initialType A : Type :=
-  | TreeStash : PBTree A -> list(nat * nat) -> initialType A.
-    
-  
-  Fixpoint initializeTree (rt : PBTree (list (nat * nat))) (stsh : list (nat * nat))
-           (l : list(nat * list nat)): option(initialType (list (nat * nat))) :=
-    
-    match rt with
-    | Leaf idx val =>
-        let data := pairGen l rt in
-        match data with
-        | [] => None
-        | h :: t => let dataH := takeL 4 data in
-                  let dataT := takeFromIdx 4 data in
-                  let newStsh := stsh ++ dataT in
-                  Some(TreeStash (list(nat * nat))(writeAtPath rt (getPath idx) dataH) newStsh)
-        end
-    | Node idx val lc rc =>
-        let data := pairGen l rt in
-        match data with
-        | [] => let dataH := takeL 4 data in
-               let dataT := takeFromIdx 4 data in
-               let newStsh := stsh ++ dataT in
-               Some(TreeStash (list (nat * nat))(writeAtPath rt (getPath idx) dataH) newStsh)
-        | h :: t => match initializeTree lc stsh l with
-                  | Some x => Some x 
-                  | None => initializeTree rc stsh l
-                  end
-        end
-    end.
-
-  Program Fixpoint getPath' (lfIdx : nat) {measure lfIdx} : list nat :=
-    match lfIdx with
-    | 0 => [0]
-    | S idx => if Nat.even idx
-              then [S idx] ++ getPath' (PeanoNat.Nat.div2 idx)
-              else [S idx] ++ getPath' (PeanoNat.Nat.div2 idx)
-    end.
-  Next Obligation.
-    apply div2.
-    Qed.
-  Next Obligation.
-    apply div2.
-    Defined.
-
-  Compute rev(getPath' 11).
-
-  Fixpoint writeatPath {A} (root: PBTree A) (path : list nat) (data: A): PBTree A :=
-    match root with
-    | Leaf idx val =>
-        match path with
-        | [] => Leaf idx data
-        | _ => Leaf idx val (* path longer than height of tree*)
-        end
-    | Node idx val l r =>
-        match path with
-        | [] => Node idx data l r
-        | h :: t => if Nat.even h
-                  then Node idx val l (writeatPath r t data)
-                  else Node idx val (writeatPath l t data) r 
-        end
-    end.
-
-  
-
-  Fixpoint clearPath (rt: PBTree (list (nat * nat ))) (l : list nat): PBTree (list(nat * nat)) := 
-    match l with
-    | [] => rt
-    | h :: t => match rt with
-              | Leaf idx val => if Nat.eqb h idx
-                             then Leaf idx []
-                             else Leaf idx val
-                                       
-              | Node idx val lc rc => if Nat.eqb h idx
-                                     then Node idx [] (clearPath lc t) (clearPath rc t)
-                                     else Node idx val (clearPath lc t) (clearPath rc t) 
-              end
-    end.
-  Compute getPath' 5.
-  Compute rev(getPath' 5).
-  Compute writeatPath PBTree1 (rev (getPath' 5)) [5;5;5].
-  Compute PBTree1.
-  Compute clearPath PBTree1 (rev(getPath' 11)).
-  Compute rev(getPath' 11).  
-
-  Inductive  NodeData: Type := Data:(nat * list BlockEntry) -> NodeData .
-
-  Fixpoint getNodeAtLevel (lvl: nat) (l: list nat) (rt: PBTree (list BlockEntry)): option NodeData:=
-    match lvl with
-    | O => match l with
-          | [] => None
-          | h :: t => match rt with
-                    | Leaf idx val => if Nat.eqb idx h
-                                     then Some (Data (idx, val))
-                                     else None
-                    | Node idx val lc rc => if Nat.eqb idx h
-                                           then Some (Data (idx, val))
-                                           else
-                                             match getNodeAtLevel lvl t lc with
-                                             | None => getNodeAtLevel lvl t rc
-                                             | Some x => Some x
-                                             end
-                    end
-          end
-    | S m => match l with
-            | [] => None
-            | h :: t => match rt with
-                      |Leaf idx val => if Nat.eqb idx h
-                                      then Some (Data (idx, val))
-                                      else None
-                      |Node idx val lc rc => if Nat.eqb idx h
-                                            then Some (Data(idx, val))
-                                            else
-                                              match getNodeAtLevel lvl t lc with
-                                              | None => getNodeAtLevel lvl t rc
-                                              | Some x => Some x
-                                              end
-                      end
-            end
-    end.
-
-  Fixpoint ReadnPopNodes (rt: PBTree (list BlockEntry)) (l: list nat) (stsh: list BlockEntry) : list BlockEntry :=
-    match l with
-    | [] => []
-    | h :: t => match rt with
-              | Leaf idx val => if Nat.eqb h idx
-                               then stsh ++ val
-                               else stsh 
-              | Node idx val lc rc => if Nat.eqb h idx
-                                     then stsh ++ val 
-                                     else stsh 
-              end
-    end.
-
-  Scheme Equality for list.
-  Scheme Equality for prod.
-
-  Print list_beq.
-  (* Definition pairEqL A B := TODO *)
-  Fixpoint posMapLookUp (bID : nat) (posMap : list(nat * nat)) :option nat :=
-    match posMap with
-    | [] => None
-    | h :: t => if Nat.eqb (fst h) bID
-              then Some (snd h)
-              else posMapLookUp bID t
-    end.
-                
-  Fixpoint retSomeVal (x : option nat) : nat :=
-    match x with
-    | None => 0
-    | Some n => n
-    end.
-
-  Fixpoint eqListPair (l1 : list BlockEntry) (l2 :  list BlockEntry) : bool :=
-    match l1 with
-    | [] => match l2 with
-           | [] => true
-           | h :: t => false
-           end
-    | x :: xs => match x with
-               | (BV f s) => 
-                   match l2 with
-                   | [] => false 
-                   | h :: t => match h with
-                             | (BV f' s') => if (andb (Nat.eqb f f') (Nat.eqb s s'))
-                                       then eqListPair xs t
-                                       else false
-                             end
-                   end
-                     
-               end
-    end.
-      
-               
-      
-  Fixpoint NodeDataEq (n1: NodeData) (n2: NodeData) : bool :=
-    match n1 with
-    | Data (x, y) =>
-        match n2 with
-        | Data (a, b) => if Nat.eqb x a
-                        then eqListPair y b
-                        else false
-        end
-    end.
-  
-
-
-  Fixpoint getCandidateBlocksHelper (rt: PBTree(list BlockEntry)) (l: list nat)
-           (lvl: nat)(bID: nat)(stsh: list BlockEntry): option BlockEntry:=
-    match getNodeAtLevel lvl l rt with (* P(x, l) *)
-    | None => None
-    | Some val =>
-        match getNodeAtLevel lvl (getPath' (retSomeVal(posMapLookUp bID position_map))) rt with (* P(position[a'],l) *)
-        | None => None
-        | Some val' => if NodeDataEq val val'
-                      then match readBlockFromStash stsh bID with
-                           | Some n => Some(BV bID n)
-                           | _ => None
-                           end
-                      else None
-        end
-    end.
-                                 
-  Fixpoint getCandidateBlocks (rt: PBTree(list BlockEntry)) (l: list nat) (lvl: nat) (stsh: list BlockEntry) : list BlockEntry :=
-    match stsh with
-    | [] => []
-    | (BV bid bdata) :: t =>
-        match getCandidateBlocksHelper rt l lvl bid stsh with
-        | None =>  (getCandidateBlocks rt l lvl t)
-        | Some v => v :: (getCandidateBlocks rt l lvl t)
-        end                     
-    end.
-
-End Tree.
-
-Section PathORAM.
-  Definition nodesTotal := 60.
-  Definition nodeCap := 4.
-  (* Definition stashInit := []. *)
-
-  Inductive Op :=
-  | Rd
-  | Wr.
-
-  Fixpoint leb (n m : nat) : bool :=
+Require Import Coq.Program.Equality.
+Require Import Lia RAM.
+
+(*** CLASSES ***)
+(* I'm rolling my own version of lots of datatypes and using typeclasses
+ * pervasively. Here are the typeclasses that support the hand-rolled datatype
+ * definitions.
+ *)
+Class Ord (A : Type) := { ord_dec : A -> A -> comparison }.
+#[export] Instance NatOrd : Ord nat := { ord_dec := Nat.compare }.
+
+Class Monoid (A : Type) :=
+  { null : A
+  ; append : A -> A -> A
+  }.
+
+Module MonoidNotation.
+  Notation "x ++ y " := (append x y) (at level 60, right associativity).
+End MonoidNotation.
+Import MonoidNotation.
+
+Class Functor (T : Type -> Type) :=
+  { map : forall {A B : Type}, (A -> B) -> T A -> T B
+  }.
+
+Class Monad (M : Type -> Type) :=
+  { mreturn : forall {A : Type}, A -> M A
+  ; mbind   : forall {A B : Type}, M A -> (A -> M B) -> M B
+  }.
+
+Module MonadNotation.
+  Notation "x <- c1 ;; c2" := (mbind c1 (fun x => c2)) 
+    (at level 100, c1 at next level, right associativity).
+
+  Notation "e1 ;; e2" := (_ <- e1 ;; e2)
+    (at level 100, right associativity).
+
+  Infix ">>=" := mbind (at level 50, left associativity).
+End MonadNotation.
+Import MonadNotation.
+
+(* user-defined well-formedness criteria for a datatype, e.g., that a dictionary
+ * represented by an association-list has sorted and non-duplicate keys
+ *)
+Class WF (A : Type) := { wf : A -> Type }.
+
+(* MISSING: correctness criteria, e.g., that `Ord` is an actual total order, etc.
+ *)
+
+(*** LISTS ***)
+
+(* #[export] Instance Functor_list : Functor list := { map := List.map }. *)
+#[export] Instance Monoid_list {A : Type} : Monoid (list A) := { null := nil ; append := @List.app A }.
+
+Fixpoint remove_list {A : Type} (p : A -> bool) (xs : list A) : list A :=
+  match xs with
+  | [] => [] 
+  | x' :: xs' =>
+      if p x'
+      then remove_list p xs'
+      else
+        x' :: remove_list p xs'
+  end.
+
+Lemma In_remove_list_In {A} (p : A -> bool) (xs : list A) : forall x,
+    In x (remove_list p xs) -> In x xs.
+Proof.
+  intros x Hx.
+  induction xs as [|y xs].
+  - destruct Hx.
+  - simpl in Hx.
+    destruct (p y).
+    + right; auto.
+    + simpl in *; tauto.
+Qed.
+
+Lemma In_remove_list_p {A} (p : A -> bool) (xs : list A) : forall x,
+    In x (remove_list p xs) -> p x = false.
+Proof.
+  intros x Hx.
+  induction xs as [|y xs].
+  - destruct Hx.
+  - simpl in Hx.
+    destruct (p y) eqn:Hy; auto.
+    destruct Hx; auto.
+    congruence.
+Qed.
+
+Lemma In_remove_list {A} (p : A -> bool) (xs : list A) : forall x,
+    In x xs -> p x = false -> In x (remove_list p xs).
+Proof.
+  intros x Hx1 Hx2.
+  induction xs as [|y xs].
+  - destruct Hx1.
+  - simpl.
+    destruct Hx1; subst.
+    + rewrite Hx2.
+      left; auto.
+    + destruct (p y); auto.
+      right; auto.
+Qed.
+
+Lemma In_remove_list_iff {A} (p : A -> bool) (xs : list A) : forall x,
+    In x (remove_list p xs) <-> In x xs /\ p x = false.
+Proof.
+  intros; split; intros.
+  - split.
+    + eapply In_remove_list_In; eauto.
+    + eapply In_remove_list_p; eauto.
+  - destruct H; eapply In_remove_list; eauto.
+Qed.
+
+(*** VECTORS ***)
+
+Definition head_vec {A : Type} {n : nat} (xs : Vector.t A (S n)) : A :=
+  match xs with
+  | Vector.cons _ x _ _ => x
+  end.
+
+Definition tail_vec {A : Type} {n : nat} (xs : Vector.t A (S n)) : Vector.t A n :=
+  match xs with
+  | Vector.cons _ _ _ xs => xs
+  end.
+
+Fixpoint zip_vec {A B : Type} {n : nat} : forall (xs : Vector.t A n) (ys : Vector.t B n), Vector.t (A * B) n :=
   match n with
-  | O =>true
+  | O => fun _ _ => Vector.nil (A * B)
+  | S n' => fun xs ys =>
+      let x := head_vec xs in
+      let xs' := tail_vec xs in
+      let y := head_vec ys in
+      let ys' := tail_vec ys in
+      Vector.cons _ (x , y) _ (zip_vec xs' ys')
+  end.
+
+Fixpoint const_vec {A : Type} (x : A) (n : nat) : Vector.t A n :=
+  match n with
+  | O => Vector.nil A
+  | S n' => Vector.cons _ x _ (const_vec x n')
+  end.
+
+Fixpoint constm_vec {A : Type} {M : Type -> Type} `{Monad M} (xM : M A) (n : nat) : M (list A) :=
+  match n with
+  | O => mreturn (@nil A)
   | S n' =>
-      match m with
-      | O => false
-      | S m' =>leb n' m'
+      x <- xM ;;
+      xs <- constm_vec xM n' ;;
+      mreturn (cons x xs)
+  end.
+
+Definition to_list_vec {A : Type} {n : nat} := @Vector.to_list A n.
+Definition map_vec {A B : Type} {n : nat} f := @Vector.map A B f n.
+
+#[export] Instance Functor_vec {n : nat} : Functor (fun A => Vector.t A n) := { map {_ _} f xs := map_vec f xs }.
+
+(*** RATIONALS ***)
+#[export] Instance Monoid_rat : Monoid Q:= { null := 0 / 1 ; append := Qplus}.
+
+(* DICTIONARIES *)
+
+(* Probably switch to `Coq.FSets.FMaps` or `ExtLib.Map.FMapAList` in a real
+ * development. Rolling your own is easy enough to do, and if you go this route
+ * you may want to enforce well-formedness and/or decideable equality of the key
+ * space via type classes.
+ *)
+
+Record dict (K V : Type) := Dict { dict_elems : list (K * V) }.
+Arguments Dict {K V} _.
+Arguments dict_elems {K V} _.
+
+Fixpoint map_alist {K V V' : Type} (f : V -> V') (kvs : list (K * V)) : list (K * V') :=
+  match kvs with
+  | nil => nil
+  | cons (k , v) kvs' => cons (k , f v) (map_alist f kvs')
+  end.
+
+Fixpoint lookup_alist {K V : Type} `{Ord K} (v : V) (k : K) (kvs : list (K * V)) :=
+  match kvs with
+  | nil => v
+  | cons (k' , v') kvs' => match ord_dec k k' with
+    | Lt => lookup_alist v k kvs'
+    | Eq => v'
+    | Gt => lookup_alist v k kvs'
+    end
+  end.
+
+Inductive wf_dict_falist {K V : Type} `{Ord K} : forall (kO : option K) (kvs : list (K * V)), Prop :=
+  | nil_WFDict : forall {kO : option K}, wf_dict_falist kO []
+  | cons_WFDict : forall {kO : option K} {k : K} {v : V} {kvs : list (K * V)},
+      match kO return Set with
+      | None => unit
+      | Some k' => ord_dec k' k = Lt
+      end
+      -> wf_dict_falist (Some k) kvs
+      -> wf_dict_falist kO ((k , v) :: kvs).
+
+Fixpoint lookup_falist {K V : Type} `{Ord K} (v : V) (k : K) (kvs : list (K * V)) :=
+  match kvs with
+  | nil => v
+  | cons (k' , v') kvs' => match ord_dec k k' with
+    | Lt => v
+    | Eq => v'
+    | Gt => lookup_falist v k kvs'
+    end
+  end.
+
+Fixpoint update_falist {K V : Type} `{Ord K} (k : K) (v : V) (kvs : list (K * V)) : list (K * V) :=
+  match kvs with
+  | nil => [ (k , v) ]
+  | cons (k' , v') kvs' => match ord_dec k k' with
+      | Lt => (k , v) :: (k' , v') :: kvs'
+      | Eq => (k , v) :: kvs'
+      | Gt => (k' , v') :: update_falist k v kvs'
       end
   end.
 
-  Definition getWriteBackBlocks (rt : PBTree(list BlockEntry))(c: nat) (l: list nat) (lvl: nat)(stsh: list BlockEntry): list BlockEntry :=
-    match List.length(stsh) with
-    | O => let candidateBlocks := @nil BlockEntry in
-          let writeBackSize := O in
-          []
-    | S m => let candidateBlocks := getCandidateBlocks rt l lvl stsh in
-            if  leb c (List.length(candidateBlocks)) 
-            then let writeBackSize := c in
-                 takeL c candidateBlocks
-            else let writeBackSize := List.length(candidateBlocks) in
-                 takeL c candidateBlocks
-    end.
-  
-  Definition st_rand := prod(Stream Z)
-                            (prod(list BlockEntry)
-                                 (PBTree(list BlockEntry))).
+#[export] Instance WF_dict {K V : Type} `{Ord K} : WF (dict K V) := { wf kvs := wf_dict_falist None (dict_elems kvs) }.
 
-  Definition triFunction leafIdx lIDs lvl (s : st_rand) : st_rand :=
-      match s with 
-      | (stream,(stsh, tr)) =>
-          let writeBackBlocks := getWriteBackBlocks tr leafIdx lIDs lvl stsh in
-          let updateStash := popStash stsh writeBackBlocks in
-          let newTree := writeToNode tr leafIdx lvl writeBackBlocks in
-          (stream, (updateStash, newTree))
-      end.
+#[export] Instance Functor_dict {K : Type} : Functor (dict K) :=
+  { map {_ _} f kvs := Dict (map_alist f (dict_elems kvs)) }.
 
-  Definition writeBacks leafIdx lIDs (lvl:nat) : state st_rand unit :=
-    let* s := get in
-    (let s' := triFunction leafIdx lIDs lvl s in
-    put s').
-    
-  Fixpoint access_rec (leafIdx: nat) (lIDs : list nat) (lvl: nat): state st_rand unit :=
-    match lvl with
-    | O => writeBacks leafIdx lIDs O 
-    | S m => let* _ := writeBacks leafIdx lIDs lvl in
-            access_rec leafIdx lIDs m 
-    end.
+Definition lookup_dict {K V : Type} `{Ord K} (v : V) (k : K) (kvs : dict K V) := lookup_falist v k (dict_elems kvs).
 
-  Print writeBacks.
-  Print access_rec.
-  Definition LEVEL := 3.
+Definition update_dict {K V : Type} `{Ord K} (k : K) (v : V) (kvs : dict K V) : dict K V :=
+  Dict (update_falist k v (dict_elems kvs)).
 
-  Definition option_get {T} (o : option T) (defaultT : T) : T :=
-    match o with
-    | Some val => val
-    | None => defaultT
-    end.
+(*** DISTRIBUTIONS ***)
 
-  Fixpoint posMapUpdate (posMap: list(nat * nat)) (nID: nat) (random: nat) : list(nat * nat) :=
-    match posMap with
-    | [] => []
-    | (b, n) :: t => if Nat.eqb b nID
-                   then (b, random) :: (posMapUpdate t nID random)
-                   else (b, n) :: (posMapUpdate t nID random)
-    end.
-      
-  Definition get_random_nat (_ : unit) : state st_rand nat :=
-    let* (stream, (stsh, tr)) := get in
-    let (random, stream') :=
-      match stream with
-      | Cons r s => (r, s)
+(* You may need to just roll your own on this one, and it will be a pain. This
+ * representation is mostly just a placeholder. This representation represents
+ * the distribution as an association list, so must be a discrete distribution
+ * with finite support. We allow multiple keys in the association list (so a
+ * multimap) because to restrict otherwise would require an `Ord` restraint on
+ * the value type, which makes it more painful to use things like the `Monad`
+ * typeclass and notation. Another way to go is to use `dict` instead of a raw
+ * association list, which has the dual trade-offs.
+ *
+ * These are extensional distributions, which make reasoning about conditional
+ * probabilities and distribution independence a pain. consider moving to
+ * intensional distributions a la the "A Language for Probabilistically
+ * Oblivious Computation" paper (Fig 10). 
+ *)
+
+Fixpoint fold_l {X Y: Type} (f : X -> Y -> Y) (b : Y) (l : list X) : Y :=
+  match l with
+  | [] => b
+  | h ::t => f h (fold_l f b t)
+  end.
+
+Definition sum_dist {A} (l : list (A * Q)) : Q := fold_l Qplus 0 (List.map snd l).
+
+Record dist (A : Type) : Type :=
+  Dist
+    { dist_pmf : list (A * Q); 
+      dist_law : Qeq (sum_dist dist_pmf) 1
+    }.
+Arguments Dist {A} _.
+Arguments dist_pmf {A} _.
+
+Definition mreturn_dist {A : Type} (x : A) : dist A.
+  refine (Dist [ (x, 1 / 1) ] _ ).
+  Proof.
+    unfold sum_dist. simpl.
+    unfold Qeq. simpl. reflexivity.
+  Defined.
+
+Lemma refold_sum_dist:
+  forall {A} (a : A) (q : Q) (l : list (A * Q)),
+    sum_dist ((a, q) :: l) = q + sum_dist l.
+Proof.
+  intros. reflexivity.
+Defined.
+
+Lemma sum_dist_app:
+  forall {A} (l1 l2 : list (A * Q)),
+    Qeq (sum_dist (l1 ++ l2)) (sum_dist l1 + sum_dist l2).
+Proof.
+  induction l1; intros.
+  - rewrite Qplus_0_l. reflexivity.
+  - simpl. destruct a. rewrite refold_sum_dist. rewrite refold_sum_dist.
+    rewrite IHl1. apply Qplus_assoc.
+Defined.
+
+Definition update_probs {B} q l :=
+  List.map
+    (fun yq' : B * Q => let (y, q') := yq' in (y, q * q'))
+    l.
+
+Lemma update_probs_OK:
+  forall {B} q l,
+    Qeq (sum_dist (@update_probs B q l)) (q * sum_dist l).
+Proof.
+  intros. induction l.
+  - unfold sum_dist. simpl. ring.
+  - destruct a. simpl. 
+    rewrite refold_sum_dist. rewrite refold_sum_dist.
+    rewrite IHl. ring.
+Defined.
+
+Definition mbind_dist_pmf {A B : Type} (xM : dist A) (f : A -> dist B) : list (B * Q) :=
+  flat_map
+   (fun (xq : A * Q) => 
+     let (x , q) := xq in 
+     (update_probs q (dist_pmf (f x))))
+   (dist_pmf xM).
+
+Definition mbind_dist {A B : Type} (xM : dist A) (f : A -> dist B) : dist B.
+ refine (Dist (mbind_dist_pmf xM f) _ ).
+Proof.
+  destruct xM. unfold mbind_dist_pmf. simpl. rewrite <- dist_law0. generalize dist_pmf0 as l. induction l.
+  - reflexivity.
+  - simpl. destruct a. rewrite refold_sum_dist. rewrite sum_dist_app.
+    remember (f a). destruct d. simpl. rewrite IHl.
+    rewrite update_probs_OK. rewrite dist_law1. ring.
+Defined.
+ 
+#[export] Instance Monad_dist : Monad dist := { mreturn {_} x := mreturn_dist x ; mbind {_ _} := mbind_dist }.
+
+Definition coin_flip : dist bool := Dist [ (true, 1 / 2) ; (false , 1 / 2) ] eq_refl.
+
+(* Definition norm_dist {A} (d: dist A) : dist A := *)
+(*   let supp := dist_pmf d in *)
+(*   let sum_tot := sum_dist d in *)
+(*   Dist(map_alist (fun x : Q => x / sum_tot) supp). *)
+
+Definition event (A : Type) := A -> bool.
+
+(* might collide when you import the List Lib. *)
+
+Fixpoint filter {A} (l: list A) (f: A -> bool): list A :=
+  match l with
+  | [] => []
+  | x :: l => if f x then x::(filter l f) else filter l f 
+  end.
+
+Fixpoint length {A} (l : list A) : nat :=
+  match l with
+    | [] => O
+    | _ :: m => S (length m)
+  end.
+
+Fixpoint takeL {A} n (l : list A) : list A :=
+  match n with
+  | O => []
+  | S m => match l with
+          | [] => []
+          | h :: t => h :: takeL m t 
+          end
+  end.
+
+(* The goal of evalDist is to evaluate the probability when given an event under a certain distribution.      *)
+
+(* 1. get the list -- dist_pmf *)
+(* 2. filter a, construct the new list (A, rat) which satisfies event predicate *)
+(* 3. reconstruct/repack a dist using this one *)
+(* 4. sum it up -- sum_dist *)
+
+ 
+Fixpoint filter_dist {A} (l: list (A * Q))
+  (f: A -> bool): list (A * Q) :=
+  match l with
+  | [] => []
+  | h :: t => 
+      match h with
+        | pair k v => 
+            if f k
+            then h :: (filter_dist t f)
+            else filter_dist t f
       end
-    in
-    let* _ := put (stream', (stsh, tr)) in
-    ret (Z.to_nat (md_tot random)).
-                     
-                              
-  (* lfIdx is always some val
-   move this to its own section*)
-
-    Definition access (op : Op) (bID : nat) (dataN : option nat) : state st_rand nat :=
-    let lfIdx_o := posMapLookUp bID position_map in
-    let lfidx := option_get lfIdx_o 0 in (* prove lfidx will not be None*)
-    let* random_nat := get_random_nat tt in
-    let position_map' := posMapUpdate position_map lfidx random_nat  in
-    let* (stream, (stsh, tr)) := get in
-
-    let* _ := put(stream, ((ReadnPopNodes tr (getPath' lfidx) stsh), tr)) in
-    let dataOld := readBlockFromStash stsh bID in
-    match op with
-    | Wr => let toPopstsh := updateStash bID (option_get dataN 0) stsh in
-           let* _ := put(stream, (toPopstsh, tr)) in
-           let* _ := access_rec lfidx (getPath' lfidx) LEVEL in
-           ret (option_get dataOld O)
-    | Rd => let* _ := access_rec lfidx (getPath' lfidx) LEVEL in
-           ret (option_get dataOld O)
-    end.
-
-  (* pos map was not recorded in the global state  *)
-End PathORAM.
-
-
-Section PathORAM.
-  Definition ValEq (a : nat) (b : nat): Prop := eq_nat a b.
-
-  Definition twoAccesses(blockId: nat ) (data: nat) : state st_rand nat :=
-    let* (stream, (stsh, tr)) := get in
-    let* _ := access Wr blockId (Some data) in
-    access Rd blockId None.
-
-  (* From QuickChick Require Import QuickChick. *)
-  (* Import QcDefaultNotation. Open Scope qc_scope. *)
-  
-  Lemma reflect_eq: forall (bID: nat), (bID =? bID) = true.
-  Proof.
-    intros.
-    induction bID.
-    - eauto.
-    - simpl. apply IHbID.
-  Qed.
-
-  Lemma posMapLookUp_some: forall (posMap: list(nat * nat)) (bID: nat) (kv: (nat * nat)),
-      eq_nat (fst kv) bID -> In kv posMap ->
-      exists v, posMapLookUp bID posMap = Some v.
-  Proof.
-    intros.
-    destruct kv. simpl in *. revert bID n n0 H H0.
-    induction posMap; intros.
-    - inversion H0.
-    - simpl in H0.
-      destruct H0 eqn:separate.
-      + subst. simpl. destruct (n =? bID) eqn: cond.
-        * exists n0. reflexivity. 
-        * apply beq_nat_false in cond.  
-        eapply eq_nat_is_eq in H.
-        rewrite H in cond. contradiction.
-      + simpl. destruct (n =? bID) eqn: cond.
-        subst; simpl. 
-        * apply beq_nat_true in cond. 
-          destruct a. simpl. destruct ( Nat.eq_dec n1 bID).
-          rewrite e.
-          pose proof (reflect_eq bID).
-          rewrite H0. exists n2. auto.
-          destruct_with_eqn (n1 =? bID). exists n2. auto.
-          specialize (IHposMap bID n n0 H i). apply IHposMap.
-        * apply beq_nat_false in cond. 
-          destruct a. simpl. destruct ( Nat.eq_dec n1 bID).
-          rewrite e.
-          pose proof (reflect_eq bID).
-          rewrite H1. exists n2. auto.
-          destruct_with_eqn (n1 =? bID). exists n2. auto.
-          specialize (IHposMap bID n n0 H i). apply IHposMap.
-  Qed.          
-      
-  
-            
-  Lemma readBlockFromStash_some:
-    forall (stsh : list BlockEntry) (bID: nat) (kv : BlockEntry), 
-      eq_nat (BlockEntry_fst kv) bID -> In kv stsh ->
-      exists v, readBlockFromStash stsh bID = Some v.
-  Proof.
-    intros.
-    destruct kv. simpl in *. revert bID f s H H0.
-    induction stsh; intros.
-    - inversion H0.
-    - simpl in H0.
-      destruct H0 eqn:separate.
-      + subst. simpl. destruct (f =? bID) eqn: cond.
-        * exists s. reflexivity. 
-        * apply beq_nat_false in cond.  
-        eapply eq_nat_is_eq in H.
-        rewrite H in cond. contradiction.
-      + simpl. destruct a.
-        destruct (f0 =? bID) eqn: cond.
-        subst; simpl. 
-        * apply beq_nat_true in cond.
-          exists s0. auto.
-        * apply beq_nat_false in cond.
-          
-          destruct ( Nat.eq_dec f0 bID). contradiction.
-          specialize (IHstsh bID f s H i).
-          auto.
-  Qed.          
-
-
-
-  
-  (* Since posMap is a dictionary, we need to have a sortedness notation over a dictionary  *)
-  Definition sortedDict (dict: list (nat * nat)) := forall i j k1 v1 k2 v2,
-      i < j ->
-      nth_error dict i = Some (k1, v1) ->
-      nth_error dict j = Some (k2, v2) ->
-      k1 = i /\ k2 = j.
-
-  Fixpoint fixedSlots (rt: PBTree (list BlockEntry)) (sz : nat) : Prop :=
-    match rt with
-    | Leaf _  idx val  => (List.length val) = sz
-    | Node _ idx val lc rc => (List.length val) = sz /\
-                               (fixedSlots lc sz) /\
-                               (fixedSlots rc sz)
-    end.
-                                                    
-  Definition posMapSimplInit (posMap : list(nat * nat)) (memSize : nat) := List.length(posMap) = memSize /\ (sortedDict posMap).
-
-  (* TODO: show PathORAM satisfies the invariant before an access and also show that it satisfies the invariant after an access.  *)
-
-  Fixpoint In_BlEntry (lbe : list BlockEntry) (key : nat) : Prop :=
-    match lbe with
-    | [] => False
-    | BV k v :: t => k = key \/ In_BlEntry t key 
-    end.
-  
-  Fixpoint In_PBTree (rt : PBTree(list BlockEntry)) (key : nat) : Prop :=
-    match rt with
-    | Leaf _ idx val => idx = key \/ False
-    | Node _ idx val lc rc =>
-        idx = key \/ In_PBTree lc key \/
-          In_PBTree rc key
-    end.
-
-  (* Print xorb. *)
-
-  (* Inductive xxor : Prop -> Prop -> Prop := *)
-  (* | f_f (x y : Prop): ~x -> ~y -> xxor x y *)
-  (* | f_t (x y : Prop): ~x -> y -> xxor x y *)
-  (* | t_f(x y : Prop): x -> ~y -> xxor x y *)
-  (* | t_t (x y : Prop): x -> y -> xxor x y. *)
-                                 
-  (* Definition invariant (stsh: list BlockEntry) (rt: PBTree (list BlockEntry)) (memSz : nat) := *)
-  (*   forall i, O <= i < memSz -> xxor (In_BlEntry stsh i) (In_PBTree rt i). *)
-
-
-  Fixpoint counting_begin (begin : nat) (lnat : list nat) : bool :=
-    match lnat with
-    | [] => true
-    | h :: t => if Nat.eqb begin h
-              then (counting_begin (S begin) t)
-              else false 
-    end.
- 
-  Fixpoint count_lst (lnat : list nat) : bool :=
-    match lnat with
-    | [] => true
-    | h :: t => (counting_begin h lnat)
-    end.
-
-  Compute count_lst [109;110;111].
-
-  Require Import Sorting.
-  Compute NatSort.sort [1;3;2].
-
-  (* get the list of block ids that live in the stash or a given path *) 
-  
-  Definition getBlockIdsFromBELst (belst : list BlockEntry) : list nat :=
-    List.map BlockEntry_fst belst.
-
-  
-  Fixpoint getBlockIdsFromPath (rt: PBTree (list BlockEntry)) (l : list nat) : list nat := 
-    match l with
-    | [] => []
-    | h :: t => match rt with
-              | Leaf _ idx val =>
-                  if Nat.eqb h idx
-                  then getBlockIdsFromBELst val
-                  else getBlockIdsFromPath rt t
-              | Node _ idx val lc rc =>
-                  if Nat.eqb h idx
-                  then (getBlockIdsFromBELst val) ++ (getBlockIdsFromPath lc t) ++
-                                                  (getBlockIdsFromPath rc t)
-                  else (getBlockIdsFromPath lc t) ++ (getBlockIdsFromPath rc t)
-              end
-    end.
-
-  Definition caterpillar (BId_stsh : list nat) (BId_path : list nat) : Prop :=
-    NoDup (NatSort.sort (BId_stsh ++ BId_path)).
-
+  end.
     
-  Definition isLeafNode (n : nat) (rt : PBTree (list BlockEntry)) : Prop :=
-    let l := (getHeight rt) in
-    (ge n (2^(l - 1))) /\ (le n (2^l - 1)).
+(* Definition evalDist {A} (x: event A) (d: dist A): Q := *)
+(*    sum_dist(Dist(filter_dist (dist_pmf d) x)). *)
 
-  Definition init_invariant
-             (s: st_rand) (memSz : nat): Prop :=
-    match s with
-    | (strm, (stsh, rt)) => 
-        forall bId posMap,
-          bId < memSz ->
-          (exists x, (isLeafNode x rt ->
-                 In bId (getBlockIdsFromPath rt (getPath' x)) \/
-                   (In bId (getBlockIdsFromBELst stsh))) /\
-                  (posMapLookUp bId posMap = (Some x)))
-    end.
-                            
+(* Definition uniform_dist {A} (l: list A) :dist A:= *)
+(*  norm_dist(Dist(map_l (fun x => (x, 1)) l)). *)
 
-  Lemma access_rec_simpl: forall leafIdx lIDs lvl, 
-      (access_rec leafIdx lIDs (S lvl)) =
-        let* _ := writeBacks leafIdx lIDs (S lvl)
-      in access_rec leafIdx lIDs lvl.
-  Proof.
-    intros.
-    reflexivity.
-  Qed.
+Fixpoint mk_n_list (n: nat):list nat :=
+  match n with
+  | O => []
+  | S n' => [n'] ++ mk_n_list n'
+  end.
 
-  Lemma runStateLemma: forall s (arSt wbSt: state st_rand unit), 
-      runState (let* _ := wbSt in arSt) s =
-        let (u', s') := runState wbSt s in runState arSt s'. 
-  Proof.
-    intros.
-    simpl.
-    reflexivity.
-  Qed.
+(* Definition coin_flip' := uniform_dist (mk_n_list 2). *)
 
-  Print mkState.
-  Print put.
+(* How to disply the distribution?  *)
 
-  Lemma runStateGetPut: forall leafIdx lIDs lvl (init_s : st_rand)
-                          (f: nat -> list nat -> nat -> st_rand -> st_rand),
-      runState (let* s := get in
-                let s' := (f leafIdx lIDs lvl s) in
-                put s') init_s =
-        runState (put (f leafIdx lIDs lvl init_s)) init_s. 
-  Proof.
-    intros.
-    simpl.
-    reflexivity.
-  Qed.
-
-  Fixpoint insert {X} (x : X) (xs : list X) (n : nat) :=
-    match xs with
-    | [] => [x]
-    | y :: ys =>
-        match n with
-        | O => x :: xs
-        | S m => y :: insert x ys m
-        end
-    end.
- 
-  Inductive parts_into {X} : list X -> list X -> list X -> Prop :=
-  | part_nil : parts_into [] [] []
-  | parts_cons_l {xs zs} {x} i ys :
-    parts_into xs ys zs ->
-    parts_into (x :: xs) (insert x ys i) zs
-  | parts_cons_r {xs ys} {x} i zs :
-    parts_into xs ys zs ->
-    parts_into (x :: xs) ys (insert x zs i).
-
-  Goal parts_into [1;2;3;4;5] [5;2] [1;4;3].
-  Proof.
-    apply (parts_cons_r 0 [4;3]).
-    apply (parts_cons_l 1 [5]).
-    apply (parts_cons_r 1 [4]).
-    apply (parts_cons_r 0 []).
-    apply (parts_cons_l 0 []).
-    constructor.
-  Qed.
-    
-  Lemma inListPartition:
-    forall {A} (a b c: list A) x, In x a \/ In x (b ++ c) -> In x (a ++ b) \/ In x c.
-  Proof.
-    intros.
-    repeat rewrite in_app_iff in *.
-    destruct H.
-    repeat left; auto.
-
-    destruct H.
-    left. right; auto.
-    right; auto.
-  Qed.
-
-  Axiom HleafNodeConst: forall x p leafIdx lvl dt,
-              isLeafNode x (writeToNode p leafIdx lvl dt) ->
-              isLeafNode x p.
-
-  Lemma zero_sum: forall s memSz leafIdx lvl dt,
-      match s with
-      |(s', (l, p)) =>
-         init_invariant s memSz ->
-         init_invariant
-           (s',
-             (popStash l dt,
-               writeToNode p leafIdx lvl dt
-             )
-           ) memSz
-      end.
-  Proof.
-    intros.
-    destruct s; destruct p.
-    intro.
-    unfold init_invariant in *.
-    intros.
-    pose proof (H bId posMap H0).
-    destruct H1. destruct H1.
-    exists x.
-    split.
-    intro.
-    eapply HleafNodeConst in H3.
-    specialize (H1 H3).
-    admit.
-    - auto.    
-    
-  Admitted.
+(* Definition cond_dist {A}(p: event A) (d: dist A) : dist A := *)
+(*   norm_dist (Dist(filter_dist (dist_pmf d) p)). *)
 
 
-  Lemma writeBacks_invariant_holds:
-    forall leafIdx lvl memSz lIDs s, 
-      init_invariant s memSz ->
-      forall u strm stsh ttr,
-        (u, (strm, (stsh, ttr))) =
-          runState (writeBacks leafIdx lIDs lvl) s -> 
-        init_invariant (strm, (stsh, ttr))  memSz.
-  Proof.
-    intros; destruct s; destruct p.
-    simpl in H0. 
-    inversion H0; subst.
-    pose proof (zero_sum (s, (l, p)) memSz leafIdx  lvl).
-    apply H1.
-    auto. 
-  Qed.  
-               
-  Lemma access_rec_invariant_holds:
-    forall (leafIdx: nat) (lIDs : list nat) (lvl:nat) (s : st_rand) (memSz : nat),
-      init_invariant s memSz ->
-      forall u strm stsh ttr,  (u, (strm, (stsh, ttr))) = runState (access_rec leafIdx lIDs lvl) s -> 
-      init_invariant (strm, (stsh, ttr)) memSz.
+(*** PATH ORAM ***)
+
+(** 
+
+  A path ORAM with depth = 2 and bucket size = 3 looks like this:
+
+  CLIENT
+  ↓↓↓↓↓↓↓↓↓↓↓↓↓↓↓↓↓↓↓↓↓↓↓↓↓↓↓↓↓↓↓↓↓↓↓↓↓↓↓↓↓↓↓↓↓↓↓↓↓↓↓↓↓↓↓↓↓↓↓↓↓↓↓
+
+  { ID ↦ PATH, …, ID ↦ PATH } ← POSITION MAP
+  {BLOCK, …, BLOCK}           ← STASH
+
+  ↑↑↑↑↑↑↑↑↑↑↑↑↑↑↑↑↑↑↑↑↑↑↑↑↑↑↑↑↑↑↑↑↑↑↑↑↑↑↑↑↑↑↑↑↑↑↑↑↑↑↑↑↑↑↑↑↑↑↑↑↑↑↑
+
+  SERVER
+  ↓↓↓↓↓↓↓↓↓↓↓↓↓↓↓↓↓↓↓↓↓↓↓↓↓↓↓↓↓↓↓↓↓↓↓↓↓↓↓↓↓↓↓↓↓↓↓↓↓↓↓↓↓↓↓↓↓↓↓↓↓↓↓
+
+                 / [ ID | PAYLOAD ] \
+                 | [ ID | PAYLOAD ] |
+                 \ [ ID | PAYLOAD ] /
+                  /               \
+                 /                 \
+                /                   \
+   / [ ID | PAYLOAD ] \   / [ ID | PAYLOAD ] \  ←
+   | [ ID | PAYLOAD ] |   | [ ID | PAYLOAD ] |  ← A BUCKET = N BLOCKS (example: N=3)
+   \ [ ID | PAYLOAD ] /   \ [ ID | PAYLOAD ] /  ←
+                            ↑↑↑↑↑↑↑↑↑↑↑↑↑↑↑↑  
+                          A BLOCK = PAIR of ID and PAYLOAD (encrypted, fixed length, e.g., 64 bits)
+
+   PATH = L (left) or R (right). For depth > 2, PATH = list of L/R (a list of bits) of length = tree depth
+
+   Note: each path is identified by a leaf of the tree
+
+  ↑↑↑↑↑↑↑↑↑↑↑↑↑↑↑↑↑↑↑↑↑↑↑↑↑↑↑↑↑↑↑↑↑↑↑↑↑↑↑↑↑↑↑↑↑↑↑↑↑↑↑↑↑↑↑↑↑↑↑↑↑↑↑
+
+  In our model we assume the parameters:
+  - tree depth:  notated l
+  - bucket size: notated n
+  And make some simplifying assumptions:
+  - block size = unbounded (PAYLOAD = ℕ)
+  - rather than representing data structures using arrays (as a real
+    implementation would), we represent directly as inductive data types
+  The objects we need to define are then:
+  - block_id     ≜ ℕ
+  - path         ≜ vector[l](𝔹)
+  - position_map ≜ block_id ⇰ path
+  - stash        ≜ list(block)
+  - bucket       ≜ vector[n](block)
+  - oram         ⩴ ⟨bucket⟩ | ⟨bucket | oram ◇ oram⟩
+  Note: we will just use association lists to represent dictionaries, e.g., for `block_id ⇰ path`.
+
+**)
+Section PORAM.
+Definition block_id := nat.
+Record block : Type := Block
+  { block_blockid : block_id
+  ; block_payload : nat
+  }.
+Definition path := list bool.
+Definition position_map := dict block_id path.
+Definition stash := list block.
+Definition bucket := list block.
+
+Variable LOP : nat.
+
+Inductive oram : Type :=
+| leaf
+| node (payload: option bucket) (o_l o_r : oram). 
+
+Fixpoint bound_pred (o : oram) (n : nat) : Prop :=
+  match o with 
+  | leaf => True
+  | node obkt g_l g_r =>
+      match obkt with
+      | Some bkt => (Nat.le (List.length bkt) n) /\ bound_pred g_l n /\ bound_pred g_r n
+      | None => bound_pred g_l n /\ bound_pred g_r n
+      end
+  end.   
+
+Definition Poram_st S M A : Type := S -> M (A * S)%type.
+
+Definition retT {S} {M} `{Monad M} {X} :
+  X -> Poram_st S M X :=
+  fun x s => mreturn (x, s).
+
+Definition bindT {S} {M} `{Monad M} {X Y} :
+  Poram_st S M X ->
+  (X -> Poram_st S M Y) ->
+  Poram_st S M Y.
+Proof.
+  unfold Poram_st.
+  intros mx f s.
+  apply (mbind (mx s)).
+  intros [x s'].
+  exact (f x s').
+Defined.
+
+Definition head_oram (o : oram) : option (list block) :=
+  match o with
+  | leaf => None
+  | node obkt _ _ => obkt
+  end.
+
+Definition tail_l_oram (o : oram) : oram :=
+  match o with
+  | leaf => leaf
+  | node  _ o_l _ => o_l
+  end.
+
+Definition tail_r_oram (o : oram) : oram :=
+  match o with
+  | leaf => leaf
+  | node _ _ o_r => o_r
+  end.
+
+Record state : Type := State
+  { state_position_map : position_map
+  ; state_stash : stash
+  ; state_oram : oram
+  }.
   
-  Proof.
-    induction lvl; intros.
-    - unfold access_rec in H0.
-      simpl in H0.
-      pose proof (writeBacks_invariant_holds leafIdx 0 memSz lIDs s H u).
-      inversion H0; subst.
-      apply H1.
-      rewrite H4. simpl. auto.
-    - rewrite access_rec_simpl in H0.
-      rewrite runStateLemma in H0.
-      remember (runState (writeBacks leafIdx lIDs (S lvl)) s) as irSt.
-      destruct irSt.
-      apply (IHlvl s0) with (u := u).
-      + destruct s0. destruct p.
-        pose proof (writeBacks_invariant_holds leafIdx (S lvl) memSz lIDs ).
-        eapply H1; eauto.
-      + eauto. 
-  Qed.    
+Definition Poram_st_get {S M} `{Monad M}: Poram_st S M S :=
+  fun s => mreturn(s,s). 
 
-  Lemma get_random_nat_invariant_holds:
-    forall s memSz,
-      init_invariant s memSz -> 
-      let (_, oldTsPair) := runState (get_random_nat tt) s in
-      init_invariant oldTsPair memSz.
-  Proof.
-    intros. 
-    destruct s as [[first_nat s] [l pb]].
-    exact H.
-  Qed.
-  
-  (* in between access_rec_invariant_holds and get_random_nat_invariant_holds there should be similar lemmas about almost every line that invariant holds.  *)
-  
-  Lemma init_invariantholds:
-    forall (memSz : nat) (op : Op) (bID : nat) (dataN : option nat) (s0 : st_rand),
-      init_invariant s0 memSz ->
-      let (_, s) := runState (access op bID dataN) s0 in
-      init_invariant s memSz.
-  Proof.
-    intros.
-    destruct s0 as [stm [sl pb]].
-    destruct op.
-    induction pb.
-    - unfold access.
-      remember ( runState
-      (let* _ := get_random_nat tt
-       in let* (stream, (stsh, tr)) := get
-          in let* _ := put (stream, (ReadnPopNodes tr (getPath' (option_get (posMapLookUp bID position_map) 0)) stsh, tr))
-             in let* _ := access_rec (option_get (posMapLookUp bID position_map) 0) (getPath' (option_get (posMapLookUp bID position_map) 0)) LEVEL
-                in ret (option_get (readBlockFromStash stsh bID) 0)) (stm, (sl, Leaf (list BlockEntry) idx val))) as oneOnion.
-      destruct oneOnion.
-      
+Definition Poram_st_put {S M} `{Monad M} (st : S) :
+  Poram_st S M unit := fun s => mreturn(tt, st).
 
-      
-    (* TODO: find all functions that mod the states in access  *)
-  Abort.
+Fixpoint get_height (o : oram) : nat :=
+  match o with
+  | leaf => 0
+  | node  _ l r => S (max (get_height l) (get_height r))
+  end.
 
 
-  (* Lemma blockEntry_in_path_or_stsh: forall memSz s0 bId dataN, *)
-  (*     init_invariant s0 memSz -> *)
-  (*     forall oldVal strm stsh pbt, *)
-  (*       (oldVal, (strm, (stsh, pbt))) := runState (access Wr bId (Some dataN)) s0 -> *)
-  (*                         readBlockFromStash stsh bId = dataN \/  *)
+Fixpoint is_p_b_tr (o : oram) (l : nat) : Prop :=
+  match o, l with
+  | leaf, O => True
+  | node _ o_l o_r, S l' =>
+      is_p_b_tr o_l l' /\ is_p_b_tr o_r l'
+  | _, _ => False
+  end.    
 
-  Definition smonad S X := S -> X * S.
-  
-  Definition state_lift {S} {X} (Inv : S -> Prop) (P : X -> Prop) : smonad S X -> Prop :=
-    fun f => forall s, Inv s -> P (fst (f s)) /\ Inv (snd (f s)).
-  
-  Definition sm_bind {S X Y} : smonad S X -> (X -> smonad S Y) -> smonad S Y :=
-    fun m f s => let (x,s') := m s in f x s'.
-    
-  Lemma bind_lift_lemma {S} {X Y} (Inv : S -> Prop) (P : X -> Prop) (Q : Y -> Prop)
-        (sx : smonad S X) (f : X -> smonad S Y) :
-    state_lift Inv P sx ->
-    (forall x, P x -> state_lift Inv Q (f x)) ->
-    state_lift Inv Q (sm_bind sx f).
-  Proof.
-    intros.
-    unfold state_lift in *.
-    simpl.
-    intros s s_inv.
-    split.
-    - unfold sm_bind.
-      destruct (sx s) eqn:Hsx.
-      specialize (H0 x).
-      apply H0.
-      + specialize (H s).
-        rewrite Hsx in H.
-        now apply H.
-      + specialize (H s).
-        rewrite Hsx in H.
-        now apply H.
-    - unfold sm_bind.
-      destruct (sx s) eqn:Hsx.
-      destruct (H s s_inv) as [Px Is0].
-      rewrite Hsx in Px; simpl in Px.
-      rewrite Hsx in Is0; simpl in Is0.
-      destruct (H0 x Px s0 Is0) as [Qx invQ].
-      auto.
+Fixpoint coord_in_bound (o : oram) (p : path) (stop: nat) : Prop :=
+  match o with
+  | leaf => False 
+  | node d_o o_l o_r =>
+      match stop with
+      | 0%nat => True 
+      | S stop' =>
+          match p with
+          | [] => False 
+          | true :: xs => coord_in_bound o_l xs stop' 
+          | false :: xs => coord_in_bound o_r xs stop'
+          end
+      end
+  end.
+
+Lemma pb_coord_in_bound : forall (o : oram) (p : path) (k lvl : nat), 
+    is_p_b_tr o (S k) ->
+    (length p) = k -> 
+    Nat.le lvl k ->
+    coord_in_bound o p lvl.
+Proof.
+  intro o.
+  induction o; simpl.
+  - intros. inversion H.
+  - intros. destruct lvl; simpl; auto.
+    destruct p; simpl in *; try lia.
+    destruct b; simpl in *.
+    + apply IHo1 with (k := (length p)); try rewrite H0.
+      tauto. reflexivity.
+      rewrite <- H0 in H1. lia.
+    + apply IHo2 with (k := (length p)); try lia.
+      destruct H. rewrite H0. auto.
 Qed.
 
-    Definition state_lift' {S} {X} (Pre : S -> Prop)(Post : S -> Prop) (P : X -> Prop) : state S X -> Prop :=
-      fun f => forall s, Pre s -> P (fst(runState f s)) /\ Post (snd (runState f s)).
+Fixpoint lookup_path_oram (o : oram) : path -> list bucket :=
+  match o with
+  | leaf => fun _ => []
+  | node obkt o_l o_r =>
+      fun p => 
+        match p with
+        | [] =>
+            match obkt with
+            | Some bkt => [bkt]
+            | None => []
+            end
+        | h :: t =>
+            match h with
+            | true => match obkt with
+                     | Some bkt => bkt :: lookup_path_oram o_l t
+                     | None => lookup_path_oram o_l t
+                     end
+            | false => match obkt with
+                      | Some bkt => bkt :: lookup_path_oram o_r t
+                      | None => lookup_path_oram o_r t
+                      end
+            end
+        end
+  end.
+
+Fixpoint clear_path (o : oram ) : path -> oram :=
+  match o with
+  | leaf => fun _ => leaf
+  | node obkt o_l o_r =>
+      fun p =>
+        match p with
+        | [] => node None o_l o_r
+        | h :: t =>
+            match h with
+            | true => node None (clear_path o_l t) o_r
+            | false => node None o_l (clear_path o_r t)
+            end
+        end
+  end.
+           
+Fixpoint makeBoolList (b : bool) (n : nat) : list bool :=
+  match n with
+  | O => []
+  | S m => b :: makeBoolList b m
+  end.
+
+Definition calc_path (id : block_id) (s : state):=
+  let l := LOP in 
+  lookup_dict (makeBoolList false l) id (state_position_map s).
+
+Definition blk_in_p (id : block_id) (v : nat) (o : oram) (p: path) := 
+  let path_blks := concat(lookup_path_oram o p) in
+  In (Block id v) path_blks.
+
+Definition blk_in_path (id : block_id) (v : nat) (s : state): Prop :=
+  blk_in_p id v (state_oram s) (calc_path id s).
+
+#[global] Instance PoramM {S M } `{Monad M} : Monad (Poram_st S M) :=
+  {|mreturn A := retT; mbind X Y := bindT |}.
+
+Definition get_State : Poram_st(state) dist(state) := Poram_st_get.
+
+Inductive operation := 
+  | Read : operation 
+  | Write : nat -> operation.
+
+Scheme Equality for list.
+Scheme Equality for prod.
+
+Definition isEqvPath (p1 p2 : path) (idx : nat) : bool := list_beq bool Bool.eqb  (takeL idx p1) (takeL idx p2).
   
-  Lemma bind_lift_lemma' {S} {X Y} (Pre: S -> Prop)(Mid : S -> Prop) (Post : S -> Prop) (P : X -> Prop) (Q : Y -> Prop)
-        (sx : state S X) (f : X -> state S Y) :
-    state_lift' Pre Mid P sx ->
-    (forall x, P x -> state_lift' Mid Post Q (f x)) ->
-    state_lift' Pre Post Q (bind sx f).
-  Admitted. 
+
+
+Definition dummy_block : block := Block O O.
+
+Fixpoint get_cand_bs (h : stash)(p : path)(stop : nat)(m : position_map) : list block :=
+  match h with
+  | [] => []
+  | x :: xs =>
+      let l := LOP in 
+      let rhs_path := lookup_dict (makeBoolList false l) (block_blockid x) m in
+      if @isEqvPath p rhs_path stop 
+      then x :: get_cand_bs xs p stop m 
+      else get_cand_bs xs p stop m 
+  end. 
+
+(* n is the capability of each node, the current magic number is 4 based on the original paper *)
+
+Definition get_write_back_blocks (p : path) (h : stash) (n : nat)(lvl : nat) (mp : position_map ) : list block :=
+  match (length h) with
+  | O => []
+  | S m => let cand_bs := get_cand_bs h p lvl mp in
+          takeL (Nat.min (length cand_bs) n ) cand_bs
+  end.
+
+Scheme Equality for nat.
+
+Fixpoint remove_aux (lst : list block) (x : block) : list block :=
+  match lst with
+  | [] => []
+  | h :: t => 
+      if andb (Nat.eqb (block_blockid h) (block_blockid x))
+           (Nat.eqb (block_payload h) (block_payload x))
+      then t 
+      else h :: (remove_aux t x)
+  end.
+
+Fixpoint remove_list_sub (sublist : list block) (lst : list block) : list block :=
+    match sublist with
+    | [] => lst
+    | h :: t => remove_list_sub t (remove_aux lst h)
+    end.
+                 
+Fixpoint lookup_ret_data (id : block_id) (lb : list block): nat :=
+  match lb with
+  | [] => 0
+  | h :: t =>
+      if Nat.eqb (block_blockid h) id then block_payload (h%nat)
+      else lookup_ret_data id t
+  end.
+
+Fixpoint up_oram_tr (o : oram) (stop : nat) (d_n : bucket) :
+  path -> oram :=
+  match o in oram return path -> oram with
+  | leaf => fun _ => leaf
+  | node d_o o_l o_r =>
+      fun p =>
+        match stop with
+        | O => node (Some d_n) o_l o_r
+        | S stop' =>
+            match p with
+            | [] => node d_o o_l o_r
+            | x :: xs =>
+                match x with
+                | true => node d_o (up_oram_tr o_l stop' d_n xs ) o_r
+                | false => node d_o o_l(up_oram_tr o_r stop' d_n xs)
+                end
+            end
+        end
+  end.
+             
+(* --- BEGIN Talia's equivalent definition of nth to reuse later --- *)
+Fixpoint nth_error_opt {A : Type} {m : nat} (v : Vector.t A m) (n : nat) : option A :=
+  match n with
+  | O =>
+    match v with
+    | Vector.nil _ => None
+    | Vector.cons _ h _ _ => Some h
+    end
+  | S p =>
+    match v with
+    | Vector.nil _ => None
+    | Vector.cons _ _ n1 t0 => nth_error_opt t0 p
+    end
+  end.
+
+Lemma nth_error_opt_some:
+  forall {A : Type} {m : nat} (v : Vector.t A m) (n : nat) (a : A),
+    nth_error_opt v n = Some a -> Nat.lt n m.
+Proof.
+  intros A m v n. revert A m v.
+  induction n; destruct v; intros; inversion H.
+  - auto with arith.
+  - specialize (IHn A n0 v a H1). auto with arith.
+Qed.
+
+Lemma fin_of_lt_irrel:
+  forall {m n : nat} (H1 H2 : Nat.lt n m), Fin.of_nat_lt H1 = Fin.of_nat_lt H2.
+Proof.
+  induction m; destruct n; intros; auto.
+  - inversion H1.
+  - inversion H1.
+  - simpl. f_equal. apply IHm.
+Qed.
+
+Lemma nth_error_OK:
+  forall {A : Type} {m : nat} (v : Vector.t A m) (n : nat) (a : A) (H : nth_error_opt v n = Some a),
+    nth_order v (nth_error_opt_some v n a H) = a.
+Proof.
+  intros A m v n. revert A m v. induction n; destruct v; intros; inversion H.
+  - subst. reflexivity.
+  - specialize (IHn A n0 v a H).
+    unfold nth_order in *. simpl in *. rewrite <- IHn. 
+    f_equal. apply fin_of_lt_irrel.
+Qed.
+(* --- END Talia's equivalent definition of nth to reuse later --- *)
+
+Definition blocks_selection (p : path) (lvl : nat) (s : state ) : state :=
+  (* unpack the state *)
+  let m := state_position_map s in (* pos_map *) 
+  let h := state_stash s in        (* stash *)
+  let o := state_oram s in         (* oram tree *)
+  let wbs := get_write_back_blocks p h 4 lvl m in (* 4 is the capability of the bucket or equivalently the number of blocks the bucket holds *)
+  let up_h := remove_list_sub wbs h in 
+  let up_o := up_oram_tr o lvl wbs p in
+  (State m up_h up_o).
+
+(* write_back is the last for-loop, searching backwards from the bottom of the tree to seek empty slots to write candidcate blocs back *)
+
+Fixpoint write_back (s : state) (p : path) (lvl : nat) : state := 
+  match lvl with
+  | O => s 
+  | S m => write_back (blocks_selection p m s) p m
+  end.
+
+Fixpoint iterate_right {X} (start : nat) (p : path) (f : path -> nat -> X -> X) (n : nat) (x : X) : X :=
+  match n with
+  | O => x
+  | S m => f p start (iterate_right (S start) p f m x)
+  end.
+
+Definition write_back_r (start : nat) (p : path) (step : nat) (s : state):=
+  iterate_right start p blocks_selection step s.
+                        
+Lemma iterate_right_split {X} n : forall (start k : nat) (f : path -> nat -> X -> X) (p : path) (x : X),
+  iterate_right start p f (n+k) x =
+  iterate_right start p f n
+  (iterate_right (n + start) p f k x).
+Proof.
+  induction n; intros.
+  - reflexivity.
+  - simpl.
+    rewrite IHn.
+    rewrite plus_n_Sm.
+    reflexivity.
+Qed.
+
+Lemma factor_lemma {X} (L k : nat) (p : path) (f : path -> nat -> X -> X) (x : X) : (k < L)%nat ->
+  iterate_right 0 p f L x =
+    iterate_right 0 p f k
+      (f p k
+         (iterate_right (S k) p f (L - 1 - k) x)
+      ).
+Proof.
+  intro.
+  assert (L = k + S ((L - 1) - k))%nat by lia.
+  rewrite H0 at 1.
+  rewrite iterate_right_split.
+  rewrite <- (plus_n_O).
+  simpl.
+  reflexivity. 
+Qed.
+
+Definition dist2Poram {S X} (dx : dist X) : Poram_st S dist X :=
+  fun st =>
+    a <- dx ;; mreturn (a, st).
+
+Fixpoint concat_option (l : list (option bucket)) : list block :=
+  match l with
+  | [] => []
+  | h :: t => match h with
+            | None => concat_option t
+            | Some v => v ++ concat_option t
+            end
+  end.
+
+Definition get_pre_wb_st (id : block_id) (op : operation) (m : position_map) (h : stash ) (o : oram) (p p_new: path) :=
+  let m' := update_dict id p_new m in
+  let bkts := lookup_path_oram o p in
+  let bkt_blocks := concat bkts in
+  let h' := bkt_blocks ++ h in
+  let h'' := remove_list 
+               (fun blk => (block_blockid blk) =? id) h' in  
+  let h''' :=
+    match op with
+    | Read => h'
+    | Write d => (Block id d) ::  h''
+    end in
+  let o' := clear_path o p in 
+  State m' h''' o'.
+
+Definition get_post_wb_st (s : state) (id_path : path):=
+  write_back_r O id_path (length id_path) s.
   
-  Definition twoAccesses2 blockId data :=
-    let* _ := access Wr blockId (Some data) in
-    access Rd blockId None. 
 
-  Lemma twoAccesses2_correct blockId data {Pre}{Mid : st_rand -> Prop} {Post} :
-    state_lift' Pre Post(eq data) (twoAccesses2 blockId data).
-  Proof.
-    unfold twoAccesses2.
-    apply (bind_lift_lemma' Pre Mid Post (fun x => x = x)).
-    -  admit.
-    -  admit. 
-Admitted. 
+Definition get_ret_data (id : block_id)(h : stash)(p : path) (o : oram):=
+  let bkts := lookup_path_oram o p in
+  let bkt_blocks := concat bkts in
+  let h' := bkt_blocks ++ h in
+  let ret_data := lookup_ret_data id h' in
+  ret_data. 
+
+Definition access (id : block_id) (op : operation) :
+  Poram_st state dist (path * nat) :=
+  PST <- get_State ;;
+  (* unpack the state *)
+  let m := state_position_map PST in
+  let h := state_stash  PST in
+  let o := state_oram PST in 
+  (* get path for the index we are querying *)
+  let len_m := LOP in
+  let p := lookup_dict (makeBoolList false len_m) id m in
+  (* flip a bunch of coins to get the new path *)      
+  p_new <- dist2Poram (constm_vec coin_flip len_m) ;;
+  (* get the updated path oram state to put and the data to return *)
+  let n_st := get_post_wb_st (get_pre_wb_st id op m h o p p_new) p in
+  let ret_data := get_ret_data id h p o in
+  (* put the updated state back *)
+  _ <- Poram_st_put n_st ;;
+  (* return the path l and the return value *)
+  mreturn((p, ret_data)).
+
+Fixpoint get_all_blks_tree (o : oram) : list block :=
+  match o with
+  | leaf => []
+  | node obkt o_l o_r => 
+      match obkt with
+      | None => get_all_blks_tree o_l ++ get_all_blks_tree o_r
+      | Some bkt => bkt ++ (get_all_blks_tree o_l ++ get_all_blks_tree o_r)
+      end
+  end.
+
+Definition disjoint_list {A} (l1 l2 : list A) :=
+  forall a, ~ (In a l1 /\ In a l2).
+
+Record well_formed (s : state ) : Prop := 
+  {
+    no_dup_stash : NoDup (List.map block_blockid (state_stash s)); 
+    no_dup_tree : NoDup (List.map block_blockid (get_all_blks_tree (state_oram s)));
+    tree_stash_disj : disjoint_list (List.map block_blockid (get_all_blks_tree (state_oram s)))
+                        (List.map block_blockid (state_stash s)); 
+    is_pb_tr : is_p_b_tr (state_oram s) (S LOP);
+    blk_in_path_in_tree :
+    forall id, 
+    let m := state_position_map s in
+    let p := lookup_dict (makeBoolList false LOP) id m in
+    let o := state_oram s in 
+    let bkts := lookup_path_oram o p in
+    let bkt_blocks := concat bkts in
+    In id (List.map block_blockid (get_all_blks_tree o)) ->
+    In id (List.map block_blockid bkt_blocks);
+    path_length : 
+    let m := (state_position_map s) in
+     let len_m := LOP in 
+     forall id, length(lookup_dict (makeBoolList false len_m) id m) = LOP;
+  }.
+
+Class PredLift M `{Monad M} := {
+  plift {X} : (X -> Prop) -> M X -> Prop;
+  lift_ret {X} : forall x (P : X -> Prop), P x -> plift P (mreturn x);
+  lift_bind {X Y} : forall (P : X -> Prop) (Q : Y -> Prop)
+    (mx : M X) (f : X -> M Y), plift P mx ->
+    (forall x, P x -> plift Q (f x)) ->
+    plift Q (mbind mx f)
+  }.
+
+(* WARNING: distribution should contain non-zero weighted support *)
+Definition dist_lift {X} (P : X -> Prop) (d : dist X) : Prop.
+Proof.   
+  destruct d.
+  eapply (Forall P (List.map fst dist_pmf0)).
+Defined.
+
+Lemma dist_lift_lemma :
+forall (X Y : Type) (P : X -> Prop)
+  (Q : Y -> Prop) (mx : dist X)
+  (f : X -> dist Y),
+dist_lift P mx ->
+(forall x : X, P x -> dist_lift Q (f x)) ->
+dist_lift Q (x <- mx;; f x).
+Proof.
+  intros. simpl mbind. unfold mbind_dist.
+    unfold dist_lift. rewrite Forall_map. unfold mbind_dist_pmf. rewrite flat_map_concat_map. rewrite Forall_concat. rewrite Forall_map.
+    eapply Forall_impl.
+    2:{destruct mx. simpl in *. rewrite Forall_map in H. exact H. }
+    intros (k,v) pk. simpl. unfold update_probs. rewrite Forall_map.
+    specialize (H0 k pk). destruct (f k). simpl in *. rewrite Forall_map in H0. eapply Forall_impl.
+    2:{exact H0. }
+    intros (a, b) pa. exact pa.
+Qed.
 
 
+#[export] Instance Pred_Dist_Lift : PredLift dist.
+refine 
+  {|
+    plift := @dist_lift;
+    lift_ret := _;
+    lift_bind := dist_lift_lemma;
+  |}.
+Proof.
+  - intros. simpl mreturn. unfold mreturn_dist. unfold dist_lift. simpl. constructor.
+    + assumption.
+    + constructor.
+Defined.
+
+Definition state_prob_lift {S} {M} `{Monad M} `{PredLift M} {X} (Pre Post : S -> Prop) (P : X -> Prop) :=
+  fun mx =>
+    forall s, Pre s -> plift (fun '(x, s') => P x /\ Post s') (mx s). 
+
+Lemma dist_lift_weaken {X} (P Q : X -> Prop) (d : dist X) :
+  (forall x, P x -> Q x) -> 
+  dist_lift P d -> dist_lift Q d.
+Proof.
+  intros.
+  unfold dist_lift in *.
+  destruct d.
+  eapply Forall_impl; eauto.
+Qed.
+
+Lemma state_prob_lift_weaken {S X} {Pre : S -> Prop} (Post : S -> Prop) {Post' : S -> Prop}
+  (P : X -> Prop) (m : Poram_st S dist X) :
+  (forall s, Post s -> Post' s) ->
+  state_prob_lift Pre Post P m ->
+  state_prob_lift Pre Post' P m.
+Proof.
+  intros.
+  unfold state_prob_lift.
+  intros.
+  unfold plift.
+  unfold Pred_Dist_Lift. simpl.
+  apply dist_lift_weaken with (P := (fun '(x, s') => P x /\ Post s')).
+  - intros.
+    destruct x. 
+    destruct H2; auto.
+  - unfold state_prob_lift in H0. apply H0.
+    apply H1.
+Qed.    
+
+Definition read_access (id : block_id) :
+  Poram_st state dist (path * nat) := access id Read.
+
+Definition write_access (id : block_id) (v : nat) :
+  Poram_st state dist (path * nat) := access id (Write v).
+
+Definition write_and_read_access (id : block_id) (v : nat) :
+  Poram_st state dist (path * nat) :=
+  bindT (write_access id v ) (fun _ => read_access id).
 
 
+Definition has_value (v : nat) : path * nat -> Prop := fun '(_, val) => v = val.
 
+(*
+ * state_prob_bind is analogous to the sequencing rule in Hoare Logic
+ *)
+Lemma state_prob_bind {S X Y} {M} `{Monad M} `{PredLift M} {Pre : S -> Prop}
+      (Mid : S -> Prop) {Post : S -> Prop} (P: X -> Prop) {Q: Y -> Prop}
+      {mx : Poram_st S M X} {f : X -> Poram_st S M Y} : 
+  state_prob_lift Pre Mid P mx ->
+  (forall x, P x -> state_prob_lift Mid Post Q (f x)) ->
+  state_prob_lift Pre Post Q (bindT mx f).
+Proof.
+  intros.
+  unfold state_prob_lift. intros.
+  eapply lift_bind; eauto.
+  intros.
+  destruct x.
+  apply H3; tauto.
+Qed.
 
+Lemma state_prob_ret {S X} {M} `{Monad M} `{PredLift M} {Pre : S -> Prop} {P : X -> Prop} {x : X}:
+  P x -> state_prob_lift Pre Pre P (retT x).
+Proof.
+  intros.
+  unfold state_prob_lift. intros.
+  unfold plift.
+  destruct H1.
+  apply lift_ret0.
+  split; auto.
+Qed.
 
+Lemma get_State_wf {Pre : state-> Prop} :
+  state_prob_lift Pre Pre Pre get_State.
+Proof.
+  intros.
+  unfold state_prob_lift; intros.
+  unfold plift.
+  simpl. 
+  apply Forall_forall.
+  intros.
+  destruct x.
+  inversion H0. inversion H1.
+  split; rewrite H4 in H3; rewrite H3 in H; auto.
+  inversion H1.
+Qed.
 
+Lemma dist2Poram_wf {X} (dx : dist X) (P : X -> Prop) {Pre : state -> Prop}:
+  dist_lift P dx ->
+  state_prob_lift Pre Pre P (dist2Poram dx).
+Proof.
+  intros. 
+  unfold state_prob_lift.
+  intros. unfold plift. unfold Pred_Dist_Lift. unfold dist_lift.
+  unfold dist2Poram. simpl. 
+  rewrite Forall_map.
+  unfold mbind_dist_pmf. rewrite flat_map_concat_map. rewrite Forall_concat.
+  rewrite Forall_map.
+  destruct dx; simpl.
+  rewrite Forall_forall; intros.
+  rewrite Forall_forall; intros.
+  destruct x0; simpl.
+  destruct p; simpl.
+  split. unfold dist_lift in H.
+  rewrite Forall_forall in H. apply H. destruct x. destruct H2. inversion H2; subst.
+  assert (Hpair : x0 = fst (x0, q0)). { simpl. reflexivity. } rewrite Hpair.
+  apply in_map; auto.
+  destruct H2.
+  destruct x. 
+  destruct H2.
+  inversion H2; subst; auto.
+  inversion H2. 
+Qed.
 
+Lemma dist_lift_coin_flip :
+  dist_lift (fun _ => True) coin_flip.
+Proof.
+  repeat constructor; auto.
+Qed.
 
+Lemma coin_flip_wf {Pre : state -> Prop} (l : nat):
+  state_prob_lift Pre Pre (fun p => length p = l) (dist2Poram (constm_vec coin_flip l)).
+Proof.
+  eapply dist2Poram_wf.
+  induction l.
+  - simpl. auto.
+  - simpl constm_vec.
+    eapply dist_lift_lemma.
+    + apply dist_lift_coin_flip.
+    + intros.
+      eapply dist_lift_lemma.
+      * exact IHl.
+      * intros. simpl in H0.
+        repeat constructor.
+        simpl in *; congruence.
+Qed.
 
+Lemma put_wf {Pre Pre' : state -> Prop} {s : state}:
+  Pre' s -> state_prob_lift Pre Pre' (fun _ => True) (Poram_st_put s).
+Proof.
+  intros.
+  unfold state_prob_lift; intros.
+  unfold plift.
+  unfold Pred_Dist_Lift.
+  unfold dist_lift.
+  unfold Poram_st_put. simpl.
+  constructor. split; auto.
+  apply Forall_nil.
+Qed.
+
+Definition get_payload (dist_a : dist (path * nat * state)): option nat :=
+  match dist_pmf dist_a with 
+  | [] => None
+  | h :: t => match h with
+            | (((_,v),_), _)  => Some v
+            end
+  end.
+             
+Definition blk_in_stash (id : block_id) (v : nat )(st : state) : Prop :=
+  let s := state_stash st in 
+  In (Block id v) s.
+
+(* kv-rel relation should hold whenever we have a write access that has (id, v) into the ORAM.   *)
+Definition kv_rel (id : block_id) (v : nat) (st : state) : Prop :=
+  (blk_in_stash id v st) \/ (blk_in_path id v st). (* "Come back to me" -- The bone dog in Shogun Studio *)
+
+ 
+Lemma remove_aux_lemma : forall (lst : list block) (a blk: block),
+    In blk lst ->
+    In blk (remove_aux lst a) \/ a = blk.
+Proof.
+  intros.
+  induction lst; intuition.
+  simpl.
+  destruct andb eqn: eq_cond; simpl.
+  - destruct H.
+    + right.
+      rewrite andb_true_iff in eq_cond.
+      do 2 rewrite Nat.eqb_eq in eq_cond.
+      rewrite <- H. destruct a, a0; f_equal; simpl in *; firstorder.
+    + tauto.
+  - destruct H.
+    + do 2 left; auto.
+    + apply IHlst in H. tauto.
+Qed.
       
-  Theorem PathORAM_simulates_RAM: forall (s0 : st_rand)(data: nat)(blockId: nat),
-      let ReadOut :=
-        (let twoAccesses :=
-           (let* _ := (access Wr blockId (Some data)) in
-            access Rd blockId None) in
-         fst (runState twoAccesses s0)
-        )
-      in ValEq data ReadOut. 
-  Proof.
-    intros. 
-    simpl.
-    pose (wrAcc := access Wr blockId (@Some nat data)).
-    destruct s0.
-    destruct p.
-    pose proof (rdAcc := access Rd blockId None).
-    unfold ValEq.    
-    unfold ReadOut.
-    unfold bind.
-    unfold Monad_state.
-    unfold runState.
-    fold wrAcc.
-    cbv zeta.
-    destruct wrAcc eqn:HwrAcc.
-    destruct (runState (s,(l,p))) eqn:HrunState.
-    Print runState.
+Lemma remove_list_sub_lemma : forall (x : block) (sub : list block) (lst : list block),
+    In x lst ->
+    In x (remove_list_sub sub lst) \/ In x sub.
+Proof.
+  intros blk s_lst.
+  induction s_lst. 
+  - simpl.  intros. left; auto.
+  - intros. simpl remove_list_sub.
+    pose proof (IHs_lst (remove_aux lst a))%list.
+    destruct (remove_aux_lemma _ a _ H).
+    + apply H0 in H1. destruct H1.
+      * left. auto.
+      * right. right; auto.
+    + right. left; auto.
+Qed.
         
-    (* Branching off: Take Chris suggestion and show that the sequence tokens are unique from each other.  *)
+Lemma kv_in_list_partition:
+  forall (id : block_id) (v : nat) (s : state) (del : list block),
+    blk_in_stash id v s ->
+    (In (Block id v)
+       (remove_list_sub del (state_stash s))  \/
+    (In (Block id v) del)).
+Proof.
+  intros.
+  unfold blk_in_stash in H.
+  apply remove_list_sub_lemma.
+  auto.
+Qed.  
+
+
+Lemma stash_path_combined_rel_Rd : forall (id : block_id) (v : nat) (s : state) (p_new : path),
+    kv_rel id v s ->
+    blk_in_stash id v ((get_pre_wb_st id Read (state_position_map s)
+                          (state_stash s)
+                          (state_oram s)
+                          (calc_path id s) p_new)).
+Proof.
+  intros.
+  unfold get_pre_wb_st. simpl.
+  apply in_or_app.
+  destruct H.
+  - right; auto.
+  - unfold blk_in_path in H. auto.
+Qed.
+
+
+Lemma stash_path_combined_rel_Wr : forall (id : block_id) (v : nat) (s : state) (p_new : path),
+    blk_in_stash id v ((get_pre_wb_st id (Write v) (state_position_map s)
+                          (state_stash s)
+                          (state_oram s)
+                          (calc_path id s) p_new)).
+Proof.
+  intros.
+  unfold get_pre_wb_st;
+  unfold blk_in_stash; simpl.
+  left; auto.
+Qed.
+
+
+Lemma write_back_split : forall lvl k p (s : state),
+    (k < lvl)%nat -> 
+    write_back_r O p lvl s =
+      write_back_r O p k 
+      ((blocks_selection p k 
+         (write_back_r (S k) p (lvl - 1 - k) s))).
+Proof.
+  unfold write_back_r.
+  intros. apply factor_lemma. auto.
+Qed.
+
+Fixpoint locate_node_in_tr (o : oram) (lvl : nat) : path -> (option bucket):=
+  match o in oram return path -> (option bucket) with
+  | leaf => fun _ => None
+  | node d o_l o_r =>
+      fun p =>
+        match lvl with
+        | O => d
+        | S lv =>
+            match p with
+            | [] => None
+            | x :: xs =>
+                match x with
+                | true => locate_node_in_tr o_l lv xs
+                | false => locate_node_in_tr o_r lv xs
+                end
+            end
+        end
+  end.
+
+Definition at_lvl_in_path (o : oram ) (lvl : nat) (p : path) (x : block) : Prop :=
+  match locate_node_in_tr o lvl p with
+  | None => False
+  | Some v => In x v
+  end.
+
+Lemma pos_map_stable_across_blk_sel : forall p lvl s,
+    state_position_map s = state_position_map (blocks_selection p lvl s).
+Proof.
+  reflexivity.
+Qed.
+
+Lemma pos_map_stable_across_wb : forall n p s start,
+    state_position_map s = state_position_map (write_back_r start p n s).
+Proof.
+  unfold write_back_r.
+  induction n; simpl; auto.
+Qed. 
+
+Lemma calc_path_pos_map_same : forall id s s',
+    state_position_map s = state_position_map s' ->
+    calc_path id s = calc_path id s'.
+Proof.
+  intros.
+  unfold calc_path.
+  congruence.
+Qed.
+
+Lemma calc_path_write_bk_r_stable : forall start id s n p ,
+    calc_path id (write_back_r start p n s) = calc_path id s.
+Proof.
+  intros.
+  apply calc_path_pos_map_same.
+  symmetry.
+  apply pos_map_stable_across_wb.
+Qed.
+
+Lemma takeL_nil : forall {X} n, @takeL X n [] = [].
+Proof.
+  induction n; simpl; auto.
+Qed.
+
+Lemma path_conversion : forall o lvl p p' b,
+    isEqvPath p p' lvl = true -> 
+    at_lvl_in_path o lvl p b -> at_lvl_in_path o lvl p' b.
+Proof.
+  induction o.
+  - intros. auto.
+  - intros.
+    destruct lvl; auto.
+    destruct p.
+    destruct p'; simpl in *; auto.
+    inversion H.
+    destruct b0. 
+    + destruct p'.  inversion H.
+      destruct b0.
+      * eapply IHo1; eauto. exact H.
+      * inversion H.
+    + destruct p'. inversion H.
+      destruct b0.
+      * inversion H.
+      * eapply IHo2; eauto. exact H.
+Qed.
+
+Lemma locate_comp_block_selection :
+  forall o p p' lvl lvl' dlt,
+    (lvl < lvl')%nat ->    
+    locate_node_in_tr (up_oram_tr o lvl dlt p') lvl' p =
+      locate_node_in_tr o lvl' p.
+Proof.
+  intro o.
+  induction o; simpl; auto.
+  - intros.
+    destruct lvl'.
+    + lia.
+    + destruct lvl; simpl in *; auto.
+      destruct p; simpl in *. 
+      * destruct p'; simpl in *; auto.
+        destruct b; simpl in *; auto.
+      * apply Arith_prebase.lt_S_n in H.
+        destruct p'; simpl; auto.
+        destruct b0, b; simpl; auto.
+Qed.
+        
+Lemma at_lvl_in_path_blocks_selection :
+  forall s p p' lvl lvl' b,
+  (lvl < lvl')%nat ->
+  at_lvl_in_path (state_oram s) lvl' p b ->
+  at_lvl_in_path (state_oram (blocks_selection p' lvl s)) lvl' p b.
+Proof.
+  intros.
+  unfold at_lvl_in_path in *.
+  unfold blocks_selection; simpl.
+  rewrite locate_comp_block_selection; auto.
+Qed.
+
+Lemma kv_in_delta_in_tree :
+  forall (o : oram) (id : block_id) (v : nat) (del : list block) (lvl: nat )(p :path),
+    In (Block id v) del ->
+    coord_in_bound o p lvl ->
+    at_lvl_in_path (up_oram_tr o lvl del p) lvl p (Block id v).
+Proof.
+  induction o; simpl in *; try contradiction. (* discharged the first case *)
+  - unfold at_lvl_in_path in *.
+    destruct lvl; simpl in *; auto.
+    + destruct p; simpl in *; auto.
+      destruct b; simpl in *.
+      * intros. apply IHo1; auto. (* yep I can tell that the IHp is not strong enough *)
+      * intros. apply IHo2; auto.
+Qed.
+
+        
+Lemma takeL_in : forall {X} (x : X) n l,
+   In x (takeL n l) -> In x l. 
+Proof.
+  induction n; intros; simpl in *.
+  - exfalso; auto.
+  - destruct l.
+    + auto.
+    + destruct H.
+      * rewrite H. left; auto.
+      * right. apply IHn. auto.
+Qed.
+
+Lemma path_eq_get_cand_bs : forall id v h p stop m,
+    In (Block id v) (get_cand_bs h p stop m) ->
+    isEqvPath p (lookup_dict (makeBoolList false LOP) id m) stop = true.
+Proof.
+  induction h; intros; simpl in *.
+  - exfalso; auto.
+  - destruct isEqvPath eqn : pEqv_cond.
+    + destruct H; simpl in *.
+      * rewrite H in pEqv_cond. auto.
+      * apply IHh. auto.
+    + apply IHh; auto.
+Qed.
+      
+Lemma stash_block_selection : forall p s id v lvl,
+    well_formed s ->
+    length p = LOP ->
+    Nat.le lvl LOP -> 
+    blk_in_stash id v s ->
+    blk_in_stash id v (blocks_selection p lvl s) \/
+      (at_lvl_in_path (state_oram
+                         (blocks_selection p lvl s)) lvl p (Block id v) /\
+         at_lvl_in_path (state_oram
+                           (blocks_selection p lvl s)) lvl (calc_path id s) (Block id v) 
+      ).
+Proof.
+  intros.
+  remember (blocks_selection p lvl s) as s'.
+  unfold blocks_selection in Heqs'.
+  unfold blk_in_stash in Heqs'.
+  unfold blk_in_stash.
+  rewrite Heqs'.
+  simpl.
+  remember (get_write_back_blocks p (state_stash s) 4 lvl (state_position_map s)) as dlt.
+  apply kv_in_list_partition with (del := dlt) in H2.  destruct H2.
+  - left; auto.
+  - right.
+    split.
+    + apply kv_in_delta_in_tree; auto.
+      apply pb_coord_in_bound with (k := LOP); auto.
+      * apply H.
+    + apply path_conversion with (p := p).
+      * rewrite Heqdlt in H2. unfold get_write_back_blocks in H2.
+        destruct (length (state_stash s)); try contradiction.
+        apply takeL_in in H2.
+        unfold calc_path.
+        apply path_eq_get_cand_bs with (v := v )(h := state_stash s); auto.
+      * apply kv_in_delta_in_tree; auto.
+        apply pb_coord_in_bound with (k := LOP); auto.
+        apply H.
+Qed.
+
+Lemma blocks_selection_wf : forall
+  (p : path) (lvl : nat) (s : state),
+  well_formed s ->
+  length p = LOP ->
+  (lvl < LOP)%nat ->
+  well_formed (blocks_selection p lvl s).
+Proof.
+Admitted.
+
+Lemma write_back_wf : forall (step start : nat) (s : state) (p : path), 
+  length p = LOP ->
+  well_formed s ->
+  Nat.le (start + step) LOP -> 
+  well_formed (write_back_r start p step  s).
+Proof.
+  induction step; intros.
+  - exact H0.
+  - apply blocks_selection_wf; auto; try lia.
+    apply IHstep; auto; lia.
+Qed.
+
+Lemma write_back_in_stash_kv_rel_aux : forall n s p id v start,
+    well_formed s ->
+    length p = LOP ->
+    Nat.le (start + n) LOP ->
+    blk_in_stash id v s ->
+    blk_in_stash id v (write_back_r start p n s) \/
+      exists k, (start <= k /\ 
+              at_lvl_in_path (state_oram (write_back_r start p n s)) k p (Block id v) /\
+              at_lvl_in_path (state_oram (write_back_r start p n s)) k (calc_path id s) (Block id v))%nat.
+Proof.
+  induction n; intros.
+  - left; auto.
+  - destruct (IHn s p id v (S start) H H0); auto; try lia.
+    + unfold write_back_r at 1.
+      simpl iterate_right at 1.
+      assert (Nat.le start LOP) by lia.
+      destruct (stash_block_selection p (write_back_r (S start) p n s) id v start) as [Hs | Hr] ; auto.
+      * apply write_back_wf; auto; try lia.
+      * right.
+        exists start; auto.
+        repeat split; auto ; try tauto.
+        destruct Hr. rewrite calc_path_write_bk_r_stable in H6.
+        exact H6.
+    + destruct H3 as [k [Hk1 Hk2]].
+      right; exists k.
+      split; [lia|].
+      unfold write_back_r; simpl iterate_right.
+      split; destruct Hk2.
+      * apply at_lvl_in_path_blocks_selection; auto.
+      * apply at_lvl_in_path_blocks_selection; auto.
+Qed. 
+
+Lemma locate_node_in_path : forall o lvl p b,
+    locate_node_in_tr o lvl p = Some b ->
+    In b (lookup_path_oram o p).
+Proof.
+  induction o.
+  - intros.
+    destruct p.
+    + inversion H.
+    + destruct b0; simpl in *; discriminate.
+  - intros.
+    destruct p.
+    + unfold locate_node_in_tr in H.
+      simpl.
+      destruct lvl; try discriminate.
+      destruct payload; 
+        inversion H; subst; try discriminate. left. auto.
+    + destruct lvl; simpl in *.
+      destruct b0; simpl.
+      destruct payload; simpl.
+      * left. inversion H. reflexivity.
+      * discriminate.
+      * destruct payload; simpl.
+        -- left. inversion H. reflexivity.
+        -- discriminate.
+      * destruct b0; simpl in *.
+        destruct payload; simpl.
+        -- right. eapply IHo1; eauto.
+        -- eapply IHo1; eauto.
+        -- destruct payload; simpl.
+           ++ right.  eapply IHo2; eauto.
+           ++ eapply IHo2; eauto.
+Qed.
+      
+Lemma weaken_at_lvl_in_path : forall o lvl p id v,
+  at_lvl_in_path o lvl p (Block id v) ->
+  blk_in_p id v o p.
+Proof.
+  intros.
+  unfold at_lvl_in_path in *.
+  destruct locate_node_in_tr eqn:?; [|tauto].
+  unfold blk_in_path.
+  unfold blk_in_p.
+  rewrite in_concat.
+  exists b. split; auto.
+  apply locate_node_in_path with (lvl := lvl); auto.
+Qed.
   
-  (* Theorem PathORAMIsSecure : *)
-  (*   forall (y : list Access) (z : list Access),  *)
-  (*    comp_indistinguish (getPos(fold_LM y)) (getPos(fold_LM z)).  *)
+Lemma write_back_in_stash_kv_rel : forall s id v p,
+    well_formed s ->
+    length p = LOP ->
+    blk_in_stash id v s ->
+    kv_rel id v (write_back_r O p (length p) s).
+Proof.
+  intros.
+  destruct (write_back_in_stash_kv_rel_aux (length p) s p id v 0 H); auto; try lia.
+  - left; auto.
+  - destruct H2 as [k [_ Hk]].
+    right.
+    eapply weaken_at_lvl_in_path.
+    rewrite calc_path_write_bk_r_stable.
+    destruct Hk.
+    eauto.
+Qed.
+
+Lemma distribute_via_get_post_wb_st : forall (id : block_id) (v : nat) (s : state) (p : path),
+    well_formed s ->
+    length p = LOP ->
+    blk_in_stash id v s -> 
+    kv_rel id v (get_post_wb_st s p).
+Proof.
+  intros.
+  unfold get_post_wb_st.
+  apply write_back_in_stash_kv_rel; simpl; auto. 
+Qed.
+
+Lemma NoDup_disjointness: forall {A B} (l1 : list A) (l2 : list A) (f : A -> B) ,
+    NoDup (List.map f l1) ->
+    NoDup (List.map f l2) ->
+    disjoint_list (List.map f l1) (List.map f l2) ->
+    NoDup (List.map f (l1 ++ l2)).
+Proof.
+  induction l1; intros; simpl; auto.
+  apply NoDup_cons.
+  - intro. rewrite map_app in H2.
+    apply in_app_or in H2.
+    destruct H2.
+    + inversion H. contradiction.
+    + apply (H1 (f a)). split; auto. left. reflexivity.
+  - apply IHl1; auto.
+    + inversion H. auto.
+    + intro. intro. unfold disjoint_list in H1.
+      apply (H1 a0).
+      destruct H2.
+      split; auto.
+      right. auto.
+Qed. 
+      
+Definition inj_on_list {A B} (l : list A) (f : A -> B) :=
+  forall x y, In x l -> In y l -> f x = f y -> x = y.
+
+Lemma NoDup_map:
+  forall A B (f: A -> B) (l: list A),
+  NoDup l -> 
+  inj_on_list l f -> 
+  NoDup (List.map f l).
+Proof.
+  intros A B f l.
+  induction l; intros.
+  - constructor.
+  - simpl; constructor.
+    + intro pf.
+      rewrite in_map_iff in pf.
+      destruct pf as [b [Hb1 Hb2]].
+      assert (a = b).
+      { apply H0.
+        * now left.
+        * now right.
+        * congruence.
+      }
+      subst.
+      inversion H; contradiction.
+    + apply IHl.
+      * inversion H; auto.
+      * intros x y Hx Hy Hxy.
+        apply H0; auto.
+        -- now right.
+        -- now right.
+Qed.
+
+Lemma NoDup_app_disj : forall {A} (l1 l2 : list A),
+    NoDup (l1 ++ l2) ->
+    disjoint_list l1 l2.
+Proof.
+  induction l1; intros; simpl in *.
+  -  unfold disjoint_list.
+     intro. intro.
+     destruct H0.
+     contradiction.
+  - intro. intro.
+    destruct H0.
+    destruct H0.
+    + rewrite H0 in H.
+      inversion H.
+      apply H4.
+      apply in_or_app.
+      right; auto.
+    + unfold disjoint_list in IHl1.
+      unfold not in IHl1.
+      apply IHl1 with (a := a0)(l2 := l2).
+      inversion H; auto.
+      split; auto.
+Qed.
+
+Lemma NoDup_app_remove_mid : forall (A : Type) (l2 l1 l3 : list A) ,
+    NoDup (l1 ++ l2 ++ l3) -> NoDup (l1 ++ l3).
+Proof.
+  induction l2; intros.
+  - exact H.
+  - apply IHl2.
+    eapply NoDup_remove_1.
+    exact H.
+Qed.    
+
+Lemma In_path_in_tree : forall o p id,
+  In id (List.map block_blockid (concat (lookup_path_oram o p))) ->
+  In id (List.map block_blockid (get_all_blks_tree o)). 
+Proof.
+  induction o; simpl; intros; auto.
+  destruct p. 
+  - destruct payload; simpl in *; auto.
+    + rewrite app_nil_r in H.
+      rewrite map_app.
+      apply in_or_app.
+      left; auto.
+    + contradiction.
+  - destruct b.
+    + destruct payload.
+      * simpl in H.
+        rewrite map_app in H.
+        apply in_app_or in H.
+        repeat rewrite map_app.
+        apply in_or_app.
+        destruct H.
+        -- left; auto.
+        -- right. apply in_or_app.
+           left. eapply IHo1; eauto.
+      * rewrite map_app. 
+        apply in_or_app.
+        left.
+        eapply IHo1; eauto.
+    + destruct payload.
+      * simpl in H.
+        rewrite map_app in H.
+        apply in_app_or in H.
+        repeat rewrite map_app.
+        apply in_or_app.
+        destruct H.
+        -- left; auto.
+        -- right. apply in_or_app.
+           right. eapply IHo2; eauto.
+      * rewrite map_app. 
+        apply in_or_app.
+        right.
+        eapply IHo2; eauto.
+Qed.
+
+Lemma NoDup_path_oram : forall o p,
+    NoDup (List.map block_blockid (get_all_blks_tree o)) ->
+    NoDup (List.map block_blockid (concat (lookup_path_oram o p))).
+Proof.
+  induction o; intros.
+  - constructor.
+  - simpl in *.
+    destruct p.
+    + destruct payload.
+      * simpl.
+        rewrite app_nil_r.
+        repeat rewrite map_app in H.
+        apply NoDup_app_remove_r in H; auto.
+      * constructor.
+    + destruct b.
+      * destruct payload.
+        -- simpl in *.
+           apply NoDup_disjointness.
+           ++ repeat rewrite map_app in H.
+              apply NoDup_app_remove_r in H; auto.
+           ++ apply IHo1.
+              repeat rewrite map_app in H.
+              apply NoDup_app_remove_l in H; auto.
+              apply NoDup_app_remove_r in H; auto.
+           ++ intros id [Hid1 Hid2].
+              apply In_path_in_tree in Hid2.
+              repeat rewrite map_app in H.
+              rewrite app_assoc in H.
+              apply NoDup_app_remove_r in H.
+              apply (NoDup_app_disj _ _ H id); split; auto.
+        -- apply IHo1.
+           rewrite map_app in H.
+           apply NoDup_app_remove_r in H; auto.
+      * destruct payload.
+        -- simpl in *.
+           apply NoDup_disjointness.
+           ++ repeat rewrite map_app in H.
+              apply NoDup_app_remove_r in H; auto.
+           ++ apply IHo2.
+              repeat rewrite map_app in H.
+              apply NoDup_app_remove_l in H; auto.
+              apply NoDup_app_remove_l in H; auto.
+           ++ intros id [Hid1 Hid2].
+              apply In_path_in_tree in Hid2.
+              repeat rewrite map_app in H.
+              apply NoDup_app_remove_mid in H.
+              apply (NoDup_app_disj _ _ H id); split; auto.
+        -- apply IHo2.
+           rewrite map_app in H.
+           apply NoDup_app_remove_l in H; auto.
+Qed. 
+
+Lemma get_all_blks_tree_clear_path_weaken : forall o id p,
+  In id (List.map block_blockid (get_all_blks_tree (clear_path o p))) ->
+  In id (List.map block_blockid (get_all_blks_tree o)).
+Proof.
+  induction o; intros.
+  - auto.
+  - destruct p; simpl in *; auto.
+    + rewrite map_app in H.
+      apply in_app_or in H.
+      destruct H.
+      * destruct payload; repeat rewrite map_app.
+        -- apply in_or_app; right.
+           apply in_or_app; left; auto.
+        -- apply in_or_app; left; auto.
+      * destruct payload; repeat rewrite map_app.
+        -- apply in_or_app; right.
+           apply in_or_app; right; auto.
+        -- apply in_or_app; right; auto.
+    + destruct b; simpl in *.
+      * rewrite map_app in H.
+        apply in_app_or in H.
+        destruct H.
+        -- destruct payload; repeat rewrite map_app.
+           ++ apply in_or_app; right.
+              apply in_or_app; left; auto.
+              eapply IHo1; eauto.
+           ++ apply in_or_app; left.
+              eapply IHo1; eauto.
+        -- destruct payload; repeat rewrite map_app.
+           ++ apply in_or_app; right.
+              apply in_or_app; right; auto.
+           ++ apply in_or_app; right; auto.
+      * destruct payload; repeat rewrite map_app.
+        -- rewrite map_app in H.
+           apply in_app_or in H.
+           destruct H.
+           ++ apply in_or_app; right.
+              apply in_or_app; left; auto.
+           ++ apply in_or_app; right.
+              apply in_or_app; right.
+              eapply IHo2; eauto.
+        -- rewrite map_app in H.
+           apply in_app_or in H.
+           destruct H.
+           ++ apply in_or_app; left; auto.
+           ++ apply in_or_app; right.
+              eapply IHo2; eauto.
+Qed.
+
+Lemma NoDup_clear_path : forall o p,
+  NoDup (List.map block_blockid (get_all_blks_tree o)) ->
+  NoDup (List.map block_blockid (get_all_blks_tree (clear_path o p))).
+Proof.
+  induction o; simpl in *; intros.
+  - apply NoDup_nil.
+  - destruct p; simpl.
+    + destruct payload; auto.
+      repeat rewrite map_app in *.
+      apply NoDup_app_remove_l in H. auto.
+    + destruct b; simpl.
+      * apply NoDup_disjointness.
+        -- destruct payload; apply IHo1.
+           ++ repeat rewrite map_app in *.
+              apply NoDup_app_remove_l in H.
+              apply NoDup_app_remove_r in H.
+              auto.
+           ++ repeat rewrite map_app in *.
+              apply NoDup_app_remove_r in H.
+              auto.
+        -- destruct payload; simpl.
+           ++ repeat rewrite map_app in *.
+              apply NoDup_app_remove_l in H.
+              apply NoDup_app_remove_l in H.
+              auto.
+           ++ repeat rewrite map_app in *.
+              apply NoDup_app_remove_l in H.
+              auto.
+        -- intros id [Hid1 Hid2].
+           apply get_all_blks_tree_clear_path_weaken in Hid1.
+           destruct payload; simpl.
+           ++ repeat rewrite map_app in *.
+              apply NoDup_app_remove_l in H.
+              eapply NoDup_app_disj. exact H.
+              split; eauto.
+           ++ repeat rewrite map_app in *.
+              eapply NoDup_app_disj. exact H.
+              split; eauto.
+      * apply NoDup_disjointness.
+        -- destruct payload; simpl.
+           ++ repeat rewrite map_app in *.
+              apply NoDup_app_remove_l in H.
+              apply NoDup_app_remove_r in H.
+              auto.
+           ++ repeat rewrite map_app in *.
+              apply NoDup_app_remove_r in H.
+              auto.
+        -- destruct payload; apply IHo2.
+           ++ repeat rewrite map_app in *.
+              apply NoDup_app_remove_l in H.
+              apply NoDup_app_remove_l in H.
+              auto.
+           ++ repeat rewrite map_app in *.
+              apply NoDup_app_remove_l in H.
+              auto.
+        -- intros id [Hid1 Hid2].
+           apply get_all_blks_tree_clear_path_weaken in Hid2.
+           destruct payload; simpl.
+           ++ repeat rewrite map_app in *.
+              apply NoDup_app_remove_l in H.
+              eapply NoDup_app_disj. exact H.
+              split; eauto.
+           ++ repeat rewrite map_app in *.
+              eapply NoDup_app_disj. exact H.
+              split; eauto.
+Qed.
+           
+Lemma get_height_stable : forall o p,
+    get_height (clear_path o p) = get_height o.
+Proof.
+  induction o; simpl; auto.
+  - destruct p.
+    simpl; auto.
+    destruct b; simpl.
+    + rewrite IHo1; auto.
+    + rewrite IHo2; auto.
+Qed.
+    
+Lemma clear_path_p_b_tree : forall o n p, 
+  is_p_b_tr o n -> 
+  is_p_b_tr (clear_path o p) n.
+Proof.
+  induction o; auto; intros.
+  destruct p.
+  - simpl.
+    destruct n.
+    + inversion H.
+    + split; destruct H; auto.
+  - destruct b; simpl.
+    destruct n.
+    + inversion H.
+    + inversion H. split.
+      * apply IHo1; auto.
+      * auto.
+    + destruct n; auto.
+      split.
+      * inversion H. auto.
+      * apply IHo2; auto. inversion H; auto.
+Qed.
+
+Lemma disj_map_inv : forall A B (l1 l2 : list A) (f : A -> B),
+  disjoint_list (List.map f l1) (List.map f l2) ->
+  disjoint_list l1 l2.
+Proof.
+  intros.
+  intros x [Hx1 Hx2].
+  apply (H (f x)); split;
+  now apply in_map.
+Qed.
+
+Lemma disj_map :
+  forall A B (f : A -> B) (l1 l2 : list A),
+    disjoint_list l1 l2 ->
+    inj_on_list (l1 ++ l2) f -> 
+    disjoint_list (List.map f l1) (List.map f l2).
+Proof.
+  intros.
+  intros x [Hx1 Hx2].
+  rewrite in_map_iff in *.
+  destruct Hx1 as [a [Ha1 Ha2]].
+  destruct Hx2 as [a' [Ha3 Ha4]].
+  assert (a = a').
+  { apply H0.
+    - apply in_or_app.
+      now left.
+    - apply in_or_app.
+      now right.
+    - congruence.
+  }
+  subst.
+  apply (H a'); tauto.
+Qed.
+
+Lemma NoDup_map_inj {A B} : forall (f : A -> B) l,
+  NoDup (List.map f l) ->
+  inj_on_list l f.
+Proof.
+  unfold inj_on_list.
+  induction l; intros nd_fl x y Hx Hy Hxy.
+  - destruct Hx.
+  - destruct Hx.
+    + destruct Hy; try congruence.
+      simpl in nd_fl.
+      rewrite NoDup_cons_iff in nd_fl.
+      destruct nd_fl as [Hfa nd].
+      elim Hfa.
+      rewrite H.
+      rewrite Hxy.
+      now apply in_map.
+    + destruct Hy.
+      * simpl in nd_fl; inversion nd_fl.
+        elim H3.
+        rewrite H0.
+        rewrite <- Hxy.
+        now apply in_map.
+      * eapply IHl; eauto.
+        now inversion nd_fl.
+Qed.
+
+Lemma inj_on_list_app : forall {A B} (l1 l2 : list A) (f : A -> B),
+    NoDup (List.map f l1) ->
+    NoDup (List.map f l2) ->
+    disjoint_list (List.map f l1) (List.map f l2) ->
+    inj_on_list (l1 ++ l2) f.
+Proof.
+  intros.
+  intros x y Hx Hy Hxy.
+  apply in_app_or in Hx.
+  apply in_app_or in Hy.
+  destruct Hx, Hy.
+  - apply (NoDup_map_inj f l1); auto.
+  - elim (H1 (f x)); split.
+    + now apply in_map.
+    + rewrite Hxy; now apply in_map.
+  - elim (H1 (f y)); split.
+    + now apply in_map.
+    + rewrite <- Hxy; now apply in_map.
+  - apply (NoDup_map_inj f l2); auto.
+Qed.
+
+
+Lemma on_path_not_off_path: forall o p id,
+  NoDup (List.map block_blockid (get_all_blks_tree o)) ->
+  In id (List.map block_blockid (concat (lookup_path_oram o p))) ->
+  ~ In id (List.map block_blockid (get_all_blks_tree (clear_path o p))).
+Proof.
+  induction o; auto; intros.
+  destruct p. 
+  - destruct payload; simpl in *.
+    + repeat rewrite map_app in *.
+      apply NoDup_app_disj in H.
+      intro Hid.
+      apply (H id); split.
+      * simpl in H0.
+        rewrite app_nil_r in H0; auto.
+      * auto.
+    + auto.
+  - destruct payload; simpl in *.
+    + destruct b; simpl in *.
+      * repeat rewrite map_app in *. (* true *)
+        apply in_app_or in H0.
+        destruct H0.
+        -- apply NoDup_app_disj in H.
+           intro Hid.
+           apply (H id); split; auto.
+           apply in_or_app.
+           apply in_app_or in Hid.
+           destruct Hid.
+           ++ left. eapply get_all_blks_tree_clear_path_weaken. exact H1.
+           ++ right. auto.
+        -- intro.
+           apply in_app_or in H1.
+           destruct H1. 
+           ++ apply (IHo1 p id); auto.
+              apply NoDup_app_remove_l in H.
+              apply NoDup_app_remove_r in H; auto.
+           ++ apply NoDup_app_remove_l in H.
+              apply NoDup_app_disj in H.
+              apply (H id); split; auto.
+              eapply In_path_in_tree. exact H0.
+      * repeat rewrite map_app in *. (* false *)
+        apply in_app_or in H0.
+        destruct H0.
+        -- apply NoDup_app_disj in H.
+           intro Hid.
+           apply (H id); split; auto.
+           apply in_or_app.
+           apply in_app_or in Hid.
+           destruct Hid.
+           ++ left. auto.
+           ++ right. eapply get_all_blks_tree_clear_path_weaken. exact H1.
+        -- intro.
+           apply in_app_or in H1.
+           destruct H1. 
+           ++ apply (IHo2 p id); auto.
+              ** apply NoDup_app_remove_l in H.
+                 apply NoDup_app_remove_l in H; auto.
+              ** apply NoDup_app_remove_l in H.
+                 apply NoDup_app_disj in H.
+                 elim (H id); split; auto.
+                 eapply In_path_in_tree; eauto.                 
+           ++ apply (IHo2 p id); auto.
+              apply NoDup_app_remove_l in H.
+              apply NoDup_app_remove_l in H; auto.
+    + destruct b; simpl in *.
+      * repeat rewrite map_app in *.
+        pose proof (H' := H).
+        apply NoDup_app_disj in H.
+        intro Hid.
+        apply (H id); split; auto.
+        -- eapply In_path_in_tree; eauto.
+        -- apply in_app_or in Hid.
+           destruct Hid; auto.
+           elim (IHo1 p id); auto.
+           apply NoDup_app_remove_r in H'; auto.
+      * repeat rewrite map_app in *.
+        pose proof (H' := H).
+        apply NoDup_app_disj in H.
+        intro Hid.
+        apply (H id); split; auto.
+        -- apply in_app_or in Hid.
+           destruct Hid; auto.
+           elim (IHo2 p id); auto.
+           apply NoDup_app_remove_l in H'; auto.
+        -- eapply In_path_in_tree; eauto.
+Qed.
+
+Lemma disjoint_list_dlt : forall o p h,
+    disjoint_list (List.map block_blockid (get_all_blks_tree o))
+      (List.map block_blockid h) ->
+    NoDup (List.map block_blockid (get_all_blks_tree o)) -> 
+    disjoint_list (List.map block_blockid (get_all_blks_tree (clear_path o p)))
+    (List.map block_blockid (concat (lookup_path_oram o p) ++ h)).
+Proof.
+  intros.
+  intros id [Hid1 Hid2].
+  rewrite map_app in *.
+  apply in_app_or in Hid2.
+  destruct Hid2.
+  - eapply on_path_not_off_path; eauto.
+  - apply (H id); split; auto.
+    eapply get_all_blks_tree_clear_path_weaken; eauto.
+Qed.
+    
+Lemma disjoint_list_sub : forall {A} (l1 l2 l3: list A),
+  (forall x, In x l1 -> In x l2) -> 
+  disjoint_list l2 l3 ->
+  disjoint_list l1 l3.
+Proof.
+  intros.
+  unfold disjoint_list in *.
+  intros. unfold not in *.
+  firstorder.
+Qed.
+
+Definition bid_in (l : list block) (x : block_id):=
+  In x (List.map block_blockid l).
+
+Lemma lookup_update_sameid : forall id m p_new, 
+    lookup_dict
+       (makeBoolList false LOP) id
+       (update_dict id p_new m) = p_new.
+Proof.
+  intros.
+  unfold lookup_dict.
+  unfold update_dict.
+  destruct m; simpl.
+  induction dict_elems0 as [|[k v] tl]; simpl.
+  - rewrite Nat.compare_refl; auto.
+  - destruct (id ?= k)%nat eqn:id_cond; simpl.
+    + rewrite Nat.compare_refl; auto.
+    + rewrite Nat.compare_refl; auto.
+    + rewrite id_cond.
+      exact IHtl.
+Qed.
+
+Lemma lookup_update_diffid : forall id id' m p_new,
+    id <> id' ->
+    lookup_dict
+      (makeBoolList false LOP)
+      id (update_dict id' p_new m) =
+      lookup_dict (makeBoolList false LOP) id m.
+Proof.
+  intros.
+  unfold lookup_dict.
+  unfold update_dict.
+  destruct m; simpl.
+  induction dict_elems0 as [|[k v] tl]; simpl.
+  - destruct (id ?= id')%nat eqn:id_cond; auto.
+    rewrite Nat.compare_eq_iff in id_cond; contradiction.
+  - destruct (id' ?= k)%nat eqn:id_cond1; simpl.
+    + rewrite Nat.compare_eq_iff in id_cond1; subst.
+      destruct (id ?= k)%nat eqn:id_cond2; auto.
+      rewrite Nat.compare_eq_iff in id_cond2; contradiction.
+    + destruct (id ?= id')%nat eqn:id_cond2; auto.
+      * rewrite Nat.compare_eq_iff in id_cond2; contradiction.
+      * rewrite <- nat_compare_lt in *.
+        assert (id < k)%nat by lia.
+        rewrite nat_compare_lt in H0.
+        rewrite H0; auto.
+    + rewrite IHtl; auto.
+Qed.
+
+Lemma lookup_off_path : forall o id p p',
+  NoDup (List.map block_blockid (get_all_blks_tree o)) ->
+  In id (List.map block_blockid (get_all_blks_tree (clear_path o p))) ->
+  In id (List.map block_blockid (concat (lookup_path_oram o p'))) ->
+  In id (List.map block_blockid (concat (lookup_path_oram (clear_path o p) p'))).
+Proof.
+  induction o; intros; simpl in *; auto.
+  destruct p; simpl in *.
+  - destruct p'.
+    + simpl.
+      destruct payload; auto.
+      repeat rewrite map_app in *.
+      apply NoDup_app_disj in H.
+      simpl in H1; rewrite app_nil_r in H1.
+      apply (H id); split; auto.
+    + destruct b.
+      * destruct payload; simpl in *; auto.
+        rewrite map_app in *.
+        apply in_app_or in H1.
+        destruct H1; auto.
+        apply NoDup_app_disj in H.
+        elim (H id); split; auto.
+        rewrite map_app; auto.
+      * destruct payload; simpl in *; auto.
+        rewrite map_app in *.
+        apply in_app_or in H1.
+        destruct H1; auto.
+        apply NoDup_app_disj in H.
+        elim (H id); split; auto.
+        rewrite map_app; auto.
+  - destruct p'.
+    + destruct payload; simpl in *.
+      * rewrite app_nil_r in H1.
+        destruct b.
+        -- simpl in *.
+           rewrite map_app in *.
+           apply NoDup_app_disj in H.
+           apply (H id); split; auto.
+           rewrite map_app.
+           rewrite in_app_iff in *.
+           destruct H0; auto.
+           left; eapply get_all_blks_tree_clear_path_weaken; eauto.
+        -- simpl in *.
+           rewrite map_app in *.
+           apply NoDup_app_disj in H.
+           apply (H id); split; auto.
+           rewrite map_app.
+           rewrite in_app_iff in *.
+           destruct H0; auto.
+           right; eapply get_all_blks_tree_clear_path_weaken; eauto.
+      * contradiction.
+    + destruct b0; simpl in *.
+      * destruct payload; simpl in *.
+        -- destruct b; simpl in *.
+           ++ repeat rewrite map_app in *.
+              apply in_app_or in H1.
+              destruct H1.
+              ** apply NoDup_app_disj in H.
+                 elim (H id); split; auto.
+                 apply in_app_or in H0.
+                 apply in_or_app.
+                 destruct H0; auto.
+                 left. eapply get_all_blks_tree_clear_path_weaken; eauto.
+              ** apply IHo1; auto.
+                 --- apply NoDup_app_remove_l in H.
+                     apply NoDup_app_remove_r in H; auto.
+                 --- apply in_app_or in H0.
+                     destruct H0; auto.
+                     apply NoDup_app_remove_l in H.
+                     apply NoDup_app_disj in H.
+                     elim (H id); split; auto.
+                     eapply In_path_in_tree; eauto.
+           ++ repeat rewrite map_app in *.
+              apply in_app_or in H1.
+              destruct H1; auto.
+              apply NoDup_app_disj in H.
+              elim (H id); split; auto.
+              apply in_or_app.
+              apply in_app_or in H0.
+              destruct H0; auto.
+              right. eapply get_all_blks_tree_clear_path_weaken; eauto.
+        -- destruct b; simpl in *; auto. 
+           repeat rewrite map_app in *.
+           apply in_app_or in H0.
+           destruct H0.
+           ++ apply IHo1; auto.
+              apply NoDup_app_remove_r in H; auto.
+           ++ apply NoDup_app_disj in H.
+              elim (H id); split; auto.
+              eapply In_path_in_tree; eauto.
+      * destruct payload; simpl in *.
+        -- destruct b; simpl in *.
+           ++ repeat rewrite map_app in *.
+              apply in_app_or in H1.
+              destruct H1; auto.
+              apply NoDup_app_disj in H.
+              elim (H id); split; auto.
+              apply in_or_app.
+              apply in_app_or in H0.
+              destruct H0; auto.
+              left. eapply get_all_blks_tree_clear_path_weaken; eauto.
+           ++ repeat rewrite map_app in *.
+              apply in_app_or in H1.
+              destruct H1; auto.
+              ** apply NoDup_app_disj in H.
+                 elim (H id); split; auto.
+                 apply in_or_app.
+                 apply in_app_or in H0.
+                 destruct H0; auto.
+                 right. eapply get_all_blks_tree_clear_path_weaken; eauto.
+              ** apply IHo2; auto.
+                 --- apply NoDup_app_remove_l in H.
+                     apply NoDup_app_remove_l in H; auto.
+                 --- apply in_app_or in H0.
+                     destruct H0; auto.
+                     apply NoDup_app_remove_l in H.
+                     apply NoDup_app_disj in H.
+                     elim (H id); split; auto.
+                     eapply In_path_in_tree; eauto.
+        -- destruct b; simpl in *; auto. 
+           repeat rewrite map_app in *.
+           apply in_app_or in H0.
+           destruct H0; auto.
+           ++ apply NoDup_app_disj in H.
+              elim (H id); split; auto.
+              eapply In_path_in_tree; eauto.
+           ++ apply IHo2; auto.
+              apply NoDup_app_remove_l in H; auto.
+Qed.
+
+Lemma rd_op_wf : forall (id : block_id) (m : position_map) (h : stash) (o : oram) (p p_new : path),
+    lookup_dict (makeBoolList false LOP) id m = p ->
+    well_formed (State m h o) -> length p_new = LOP -> 
+    well_formed
+      {|
+        state_position_map := update_dict id p_new m;
+        state_stash := (concat (lookup_path_oram o p) ++ h)%list;
+        state_oram := clear_path o p
+      |}.
+Proof.
+  intros.
+  destruct H0.
+  constructor; simpl in *.
+  - apply NoDup_disjointness.
+    + apply NoDup_path_oram. auto.
+    + auto.
+    + apply disjoint_list_sub with
+        (l2 := List.map block_blockid (get_all_blks_tree o)); auto.
+      intros. apply In_path_in_tree with (p := p). exact H0.
+  - apply NoDup_clear_path. auto.
+  - apply disjoint_list_dlt. auto. auto.
+  - apply clear_path_p_b_tree. auto.
+  - intros id' Hid'.
+    destruct (id =? id') eqn:id_cond.
+    + rewrite Nat.eqb_eq in id_cond. 
+      rewrite <- id_cond in *; clear id_cond.
+      pose (get_all_blks_tree_clear_path_weaken _ _ _ Hid') as Hid'2.
+      specialize (blk_in_path_in_tree0 id Hid'2).
+      rewrite H in blk_in_path_in_tree0; clear Hid'2.
+      elim on_path_not_off_path with (id := id) (o := o) (p := p); auto.
+    + rewrite Nat.eqb_neq in id_cond.
+      rewrite lookup_update_diffid; auto.
+      apply lookup_off_path; auto.
+      apply blk_in_path_in_tree0.
+      eapply get_all_blks_tree_clear_path_weaken; eauto.
+  - intro.
+    destruct (Nat.eqb id id0) eqn : id_cond.
+    + rewrite Nat.eqb_eq in id_cond. rewrite id_cond. rewrite lookup_update_sameid.
+      auto.
+    + rewrite lookup_update_diffid. auto.
+      rewrite Nat.eqb_neq in id_cond. auto.
+Qed.
+
+Lemma not_in_removed : forall l id,
+ ~ In id
+  (List.map block_blockid
+     (remove_list (fun blk : block => block_blockid blk =? id)
+        l)).
+Proof.
+  intros.
+  rewrite in_map_iff.
+  intros [b [Hb1 Hb2]].
+  rewrite In_remove_list_iff in Hb2.
+  destruct Hb2 as [_ Hb2].
+  rewrite Hb1 in Hb2.
+  simpl in Hb2.
+  rewrite Nat.eqb_neq in Hb2.
+  contradiction.
+Qed.
+
+Lemma NoDup_remove_list : forall l id,
+    NoDup (List.map block_blockid l) -> 
+    NoDup
+      (List.map block_blockid
+         (remove_list (fun blk : block => block_blockid blk =? id)
+            l)).
+Proof.
+  induction l; simpl; intros; auto.
+  destruct (block_blockid a =? id).
+  - apply IHl; auto.
+    inversion H; auto.
+  - simpl.
+    constructor.
+    + intro pf.
+      rewrite in_map_iff in pf.
+      destruct pf as [b [Hb1 Hb2]].
+      rewrite In_remove_list_iff in Hb2.
+      destruct Hb2 as [Hb2 Hb3].
+      inversion H.
+      rewrite <- Hb1 in H2.
+      apply H2.
+      apply in_map; auto.
+    + apply IHl.
+      inversion H; auto.
+Qed.
+      
+Lemma wr_op_wf : forall (id : block_id) (v : nat) (m : position_map) (h : stash) (o : oram) (p p_new : path),
+    well_formed (State m h o) -> length p_new = LOP ->
+    lookup_dict (makeBoolList false LOP) id m = p ->
+    well_formed
+    {|
+      state_position_map := update_dict id p_new m;
+      state_stash :=
+        {| block_blockid := id; block_payload := v |}
+        :: remove_list (fun blk : block => block_blockid blk =? id)
+             (concat (lookup_path_oram o p) ++ h);
+      state_oram := clear_path o p
+    |}.
+Proof.
+  intros.
+  destruct H.
+  constructor; simpl in *.
+  - rewrite NoDup_cons_iff; split.
+    + apply not_in_removed.
+    + apply NoDup_remove_list.
+      apply NoDup_disjointness; auto.
+      * apply NoDup_path_oram; auto.
+      * eapply disjoint_list_sub.
+        -- apply In_path_in_tree.
+        -- auto.
+  - apply NoDup_clear_path. auto.
+  - intros id' [Hid'1 Hid'2].
+    destruct Hid'2.
+    + rewrite <- H in Hid'1; clear H.
+      apply on_path_not_off_path with (id := id) (o := o) (p := p); auto.
+      rewrite <- H1.
+      apply blk_in_path_in_tree0.
+      eapply get_all_blks_tree_clear_path_weaken; eauto.
+    + eapply disjoint_list_dlt; eauto; split; eauto.
+      rewrite in_map_iff in *.
+      destruct H as [b [Hb1 Hb2]].
+      exists b; split; auto.
+      rewrite In_remove_list_iff in Hb2; destruct Hb2; auto.
+  - apply clear_path_p_b_tree. auto.
+  - intros id' Hid'.
+    destruct (id =? id') eqn:id_cond.
+    + rewrite Nat.eqb_eq in id_cond. 
+      rewrite <- id_cond in *; clear id_cond.
+      pose (get_all_blks_tree_clear_path_weaken _ _ _ Hid') as Hid'2.
+      specialize (blk_in_path_in_tree0 id Hid'2).
+      rewrite H1 in blk_in_path_in_tree0; clear Hid'2.
+      elim on_path_not_off_path with (id := id) (o := o) (p := p); auto.
+    + rewrite Nat.eqb_neq in id_cond.
+      rewrite lookup_update_diffid; auto.
+      apply lookup_off_path; auto.
+      apply blk_in_path_in_tree0.
+      eapply get_all_blks_tree_clear_path_weaken; eauto.
+  - intro.
+    destruct (Nat.eqb id id0) eqn : id_cond.
+    + rewrite Nat.eqb_eq in id_cond. rewrite id_cond. rewrite lookup_update_sameid.
+      auto.
+    + rewrite lookup_update_diffid. auto.
+      rewrite Nat.eqb_neq in id_cond. auto.
+Qed.
+
+Lemma get_pre_wb_st_wf : forall (id : block_id) (op : operation) (m : position_map) (h : stash) (o : oram) (p p_new : path),
+    well_formed (State m h o) ->
+    length p_new = LOP ->
+    lookup_dict (makeBoolList false LOP) id m = p ->    
+    well_formed (get_pre_wb_st id op m h o p p_new).
+Proof.
+  intros.
+  unfold get_pre_wb_st.
+  destruct op. 
+  - simpl. apply rd_op_wf; auto.
+  - simpl. apply wr_op_wf; auto.
+Qed.
+
+Lemma get_post_wb_st_wf : forall (s : state) (p : path),
+    well_formed s ->
+    length p = LOP ->
+    well_formed (get_post_wb_st s p).
+Proof.
+  intros.
+  unfold get_post_wb_st.
+  apply write_back_wf; auto; lia.
+Qed.
+
+Lemma zero_sum_stsh_tr_Wr
+  (s : state) (id : block_id) (v : nat) (p p_new : path):
+  well_formed s ->
+  length p = LOP ->
+  length p_new = LOP ->
+  kv_rel id v
+    (get_post_wb_st
+       (get_pre_wb_st id (Write v)
+          (state_position_map s) (state_stash s) (state_oram s)
+          (calc_path id s) p_new) p).
+Proof.
+  intros.
+  apply distribute_via_get_post_wb_st; auto.
+  - apply get_pre_wb_st_wf; auto.
+    destruct s; auto.
+  - apply stash_path_combined_rel_Wr.
+Qed.
+
+Lemma blk_in_path_in_lookup_oram : forall (id : block_id) (v : nat) (s : state) ,
+    blk_in_path id v s -> 
+    In (Block id v)
+      (concat
+         (lookup_path_oram (state_oram s)
+            (calc_path id s)
+         )
+      ).
+Proof.
+  intros.
+  unfold blk_in_path in H.
+  unfold calc_path. auto.
+Qed.
+
+        
+Lemma zero_sum_stsh_tr_Rd_rev :
+  forall (id : block_id) (v : nat) (s : state) (p p_new : path),
+    well_formed s ->
+    length p = LOP ->
+    length p_new = LOP -> 
+    kv_rel id v s  -> 
+    kv_rel id v (get_post_wb_st
+      (get_pre_wb_st id Read (state_position_map s)
+         (state_stash s)
+         (state_oram s)
+         (calc_path id s) p_new) p). 
+Proof.
+  intros.
+  apply distribute_via_get_post_wb_st; auto.
+  - apply get_pre_wb_st_wf; auto. destruct s; auto.
+  - apply stash_path_combined_rel_Rd. auto.
+Qed.
+  
+Lemma lookup_ret_data_block_in_list (id : block_id) (v : nat) (l : list block) :
+  NoDup (List.map block_blockid l) ->
+  In (Block id v) l -> lookup_ret_data id l = v.
+Proof.
+  intro ND.
+  intros.
+  induction l; simpl; try contradiction.
+  destruct (block_blockid a =? id) eqn: id_cond.
+  - destruct H; simpl in *.
+    + rewrite H; auto.
+    + inversion ND; subst.
+      rewrite Nat.eqb_eq in id_cond.
+      rewrite id_cond in H2.
+      apply List.in_map with (f := block_blockid) in H.
+      simpl in *. contradiction.
+  - apply IHl.
+    + inversion ND; auto.
+    + destruct H; auto.
+      rewrite H in id_cond. simpl in *. rewrite Nat.eqb_neq in id_cond.
+      contradiction.
+Qed.
+
+Lemma zero_sum_stsh_tr_Rd (id : block_id) (v : nat) (m : position_map) (h : stash) (o : oram) :
+  well_formed (State m h o) ->
+  kv_rel id v (State m h o) ->
+  get_ret_data id h (calc_path id (State m h o)) o = v.
+Proof.
+  simpl.
+  intros.
+  destruct H0. 
+  - (* assume in stash *)
+    apply lookup_ret_data_block_in_list.
+    + apply NoDup_disjointness; try repeat apply H.
+      * apply NoDup_path_oram. apply H.
+      * destruct H.
+        apply disjoint_list_sub with
+        (l2 := List.map block_blockid (get_all_blks_tree o)); auto.
+        intros. eapply In_path_in_tree. exact H.
+    + apply in_or_app. right. auto.
+  - (* assume in path *)
+    apply lookup_ret_data_block_in_list.
+    + apply NoDup_disjointness; try repeat apply H.
+      * apply NoDup_path_oram. apply H.
+      * destruct H.
+        apply disjoint_list_sub with
+          (l2 := List.map block_blockid (get_all_blks_tree o)); auto.
+        intros. eapply In_path_in_tree. exact H.
+    + unfold blk_in_path in H. simpl in *.
+    apply in_or_app. left. auto.
+Qed.
+
+Lemma read_access_wf (id : block_id)(v : nat) :
+  state_prob_lift (fun st => @well_formed st /\ kv_rel id v st) (fun st => @well_formed st /\ kv_rel id v st) (has_value v) (read_access id).
+Proof.
+  remember (fun st : state => well_formed st /\ kv_rel id v st) as Inv. 
+  apply (state_prob_bind Inv Inv).
+  - apply get_State_wf.
+  - intros.
+    apply (state_prob_bind Inv (fun p => length p = LOP)).
+    + apply coin_flip_wf.
+    + intros. simpl.
+      apply (state_prob_bind Inv (fun _ => True)).
+      * apply put_wf. rewrite HeqInv in H; destruct H.
+        rewrite HeqInv. split.
+        -- apply get_post_wb_st_wf; [|apply H].
+           apply get_pre_wb_st_wf; auto. destruct x. exact H.
+        -- apply zero_sum_stsh_tr_Rd_rev; auto. apply H. 
+      * intros. rewrite HeqInv. apply state_prob_ret.
+        rewrite HeqInv in H. destruct H. simpl.
+        symmetry. apply zero_sum_stsh_tr_Rd; destruct x; auto.
+Qed. 
+
+Lemma write_access_wf (id : block_id) (v : nat) :
+  state_prob_lift (fun st => @well_formed st) (fun st => @well_formed st /\ kv_rel id v st) (fun _ => True) (write_access id v).
+Proof.
+  remember (fun st : state => well_formed st) as Inv.
+  apply (state_prob_bind Inv Inv).
+  - apply get_State_wf.
+  - intros.
+    rewrite HeqInv in H.
+    apply (state_prob_bind Inv (fun p => length p = LOP)).
+    + apply coin_flip_wf.
+    + intros. simpl.
+      apply (state_prob_bind (fun st => @well_formed st /\ kv_rel id v st) (fun _ => True)).
+      * apply put_wf; simpl; split.
+        apply get_post_wb_st_wf; auto.
+        -- apply get_pre_wb_st_wf; auto. destruct x; exact H.
+        -- apply H.
+        -- apply zero_sum_stsh_tr_Wr; auto. 
+           apply H.
+      * intros. rewrite HeqInv. eapply state_prob_ret. auto.
+Qed. 
+
+(*
+ * this lemma is saying that the write_and_read_access preserves the well-formedness invariant
+ * and returns the correct value
+ *)
+
+Lemma write_and_read_access_lift (id : block_id)(v : nat):
+  state_prob_lift (@well_formed) well_formed (has_value v)
+                  (write_and_read_access id v).
+Proof.
+  apply (state_prob_bind
+           (fun st => well_formed st /\ kv_rel id v st)
+           (fun _ => True)).
+  - eapply write_access_wf.
+  - intros _ _.
+    apply (state_prob_lift_weaken (fun st : state => well_formed st /\ kv_rel id v st)).
+    + tauto.
+    + apply read_access_wf.
+Qed.
+
+Lemma extract_payload (id : block_id) (v: nat) (s : state) : 
+  plift (fun '(x, s') => has_value v x /\ well_formed s') (write_and_read_access id v s) -> 
+  get_payload (write_and_read_access id v s) = Some v.
+Proof.
+  intros ops_on_s.
+  destruct (write_and_read_access id v s). unfold get_payload.
+  simpl in *. destruct dist_pmf0.
+  - simpl in *. inversion dist_law0.
+  - simpl in *.  destruct p.  destruct p.  destruct p. simpl in ops_on_s. inversion ops_on_s.
+    destruct H1. simpl in H1. congruence.
+Qed. 
+
+Theorem PathORAM_simulates_RAM (id : block_id) (v : nat) (s : state) :
+  well_formed s ->
+    get_payload(write_and_read_access id v s) = Some v.
+Proof.
+  intros wf_s.
+  apply extract_payload.
+  apply write_and_read_access_lift. auto.
+Qed.
+
+End PORAM.
+
+Module Dist_State <: StateMonad.
+  Definition state S X := dist (X * S).
+  Definition State S X := Poram_st S dist X.
+
+  Definition ret {S X} := @retT S dist _ X.
+  Definition bind {S X} := @bindT S dist _ X.
+  Definition get {S} := @Poram_st_get S dist _.
+  Definition put {S} := @Poram_st_put S dist _.
+End Dist_State.
+
+(* Path ORAM is a RAM (functional correctness specification, WIP) *)
+Module PathORAM <: RAM (Dist_State).
+
+  Definition K := block_id.
+  Definition V := nat.
+  Definition S : Type := state. 
+  Definition Vw (V : Type) := prod path V.
+
+  Module M := Dist_State.
+  Definition bind {X Y} := @M.bind S X Y.
+  Definition ret {X} := @M.ret S X.
+  Definition get := @M.get S.
+  Definition put := @M.put S.
+
+  Definition well_formed s := 
+    let o := state_oram s in
+    let len_m := get_height o in
+    well_formed (pred len_m) s.
+
+  Definition write k v := 
+      PST <- get_State ;;
+      let o := state_oram PST in
+      let len_m := get_height o in
+      write_access (pred len_m) k v.
+
+  Definition read k :=
+    PST <- get_State ;;
+    let o := state_oram PST in
+    let len_m := get_height o in
+    read_access (pred len_m) k.
+
+  Definition wrap v : Vw V := ([], v). (* path doesn't matter for this *)
+
+  Definition get_payload (s : M.state S (Vw V)) :=
+   @get_payload s.
+
+  Lemma read_and_read_lemma (k : K) (s : S):
+    @state_prob_lift state dist Monad_dist Monad_dist Pred_Dist_Lift (Vw V) 
+      well_formed 
+      well_formed
+      (fun v => eq (get_payload (bind (read k) ret s)) (Some (snd v)))
+      (bind (read k) (fun _ => read k)).
+  Proof.
+    unfold state_prob_lift. intros. admit. (* TODO *)
   Admitted.
+
+  Lemma extract_payload_read_read k (s : state) : 
+    plift
+      (fun '(x, s') => get_payload (bind (read k) ret s) = Some (snd x) /\ well_formed s')
+      (bind (read k) (fun _ => read k) s) -> 
+    get_payload (bind (read k) (fun _ => read k) s) = get_payload ((bind (read k) ret) s).
+  Proof.
+    intros. destruct (bind (read k) (fun _ => read k) s). destruct (bind (read k) ret s).
+    unfold get_payload, PathORAM_typeclass.get_payload. 
+    destruct dist_pmf0, dist_pmf1; try discriminate.
+    simpl in *. destruct p. destruct p. destruct p. destruct p0. destruct p0. destruct p0.
+    simpl in H. inversion H. destruct H2. simpl in *.
+    rewrite <- H2. reflexivity.
+  Qed.
+
+  Definition opt_lift {X} (P : X -> Prop) : option X -> Prop :=
+    fun o =>
+      match o with
+      | None => False
+      | Some x => P x
+      end.
+
+  Lemma lift_payload {Pre Post : state -> Prop} {P : nat -> Prop} 
+    (m : Poram_st S dist (path * nat)) s :
+    Pre s ->
+    state_prob_lift Pre Post (fun '(_,x) => P x) m ->
+    opt_lift P (PathORAM_typeclass.get_payload (m s)).
+  Proof.
+    intros Hs Hm.
+    unfold opt_lift.
+    unfold PathORAM_typeclass.get_payload.
+    specialize (Hm s Hs).
+    destruct (m s); simpl.
+    destruct dist_pmf0.
+    - discriminate.
+    - destruct p. destruct p. destruct p.
+      inversion Hm; tauto.
+  Qed.
+
+  Lemma is_p_b_tr_height : forall o n,
+    is_p_b_tr o n ->
+    get_height o = n.
+  Proof.
+    induction o; intros n Ho; simpl in *.
+    - destruct n; auto.
+      contradiction.
+    - destruct n; destruct Ho.
+      rewrite (IHo1 n); auto.
+      rewrite (IHo2 n); auto.
+      rewrite Nat.max_id; auto.
+  Qed.
+
+  Lemma get_height_wf : forall LOP s,
+    PathORAM_typeclass.well_formed LOP s ->
+    get_height (state_oram s) = Datatypes.S LOP.
+  Proof.
+    intros LOP s Hs.
+    apply is_pb_tr in Hs.
+    apply is_p_b_tr_height; auto.
+  Qed.
+
+  Lemma read_and_write_compat_lemma_1_aux :
+    forall LOP k v s,
+      PathORAM_typeclass.well_formed LOP s ->
+      get_payload ((bind (write k v) (fun _ => read k)) s) =
+      get_payload (write_and_read_access LOP k v s).
+  Proof.
+    intros LOP k v s wf_s.
+    rewrite PathORAM_simulates_RAM; auto.
+    assert (opt_lift (eq v) (get_payload (bind (write k v) (fun _ => read k) s))).
+    { eapply lift_payload; eauto.
+      eapply state_prob_bind.
+      + unfold write.
+        eapply state_prob_bind.
+        * apply get_State_wf.
+        * intros s' wf_s'.
+          rewrite get_height_wf with (LOP := LOP); auto.
+          apply write_access_wf.
+      + intros _ _.
+        unfold read.
+        eapply state_prob_bind.
+        * apply get_State_wf.
+        * simpl; intros s' [wf_s' Hkv].
+          rewrite get_height_wf with (LOP := LOP); auto.
+          apply read_access_wf.
+    }
+    unfold opt_lift in H.
+    destruct get_payload; auto. contradiction.
+  Qed.
+
+  Lemma read_and_write_compat_lemma_1 :
+    forall k v s,
+      well_formed s ->
+      get_payload ((bind (write k v) (fun _ => read k)) s) =
+      get_payload (write_and_read_access (pred (get_height (state_oram s))) k v s).
+  Proof.
+    intros k v s wf_s.
+    apply read_and_write_compat_lemma_1_aux.
+    exact wf_s.
+  Qed.
+
+  Lemma read_and_write_compat_lemma_2 :
+    forall k v s,
+      get_payload ((bind (write k v) (fun _ => ret (wrap v))) s) = Some v.
+    Proof.
+      intros. unfold get_payload. unfold PathORAM_typeclass.get_payload.
+      destruct (bind (write k v) (fun _ : path * nat => ret (wrap v)) s) eqn:?.
+      simpl. destruct dist_pmf0.
+      - discriminate.
+      - destruct p. destruct p. destruct v0. f_equal.
+        unfold bind in Heqd. unfold M.bind in Heqd. 
+        unfold bindT in Heqd. destruct (write k v s) eqn:?.
+        simpl in Heqd. inversion Heqd. unfold mbind_dist_pmf in H0.
+        simpl in H0. destruct dist_pmf1.
+        + discriminate.
+        + simpl in H0. destruct p0. simpl in H0. destruct p0. simpl in H0.
+         unfold wrap in H0. inversion H0. reflexivity.
+    Qed.
+
+  (* --- RAM laws --- *)
+
+  Theorem read_read :
+    forall (k : K) (s : S), 
+      well_formed s ->
+      get_payload ((bind (read k) (fun _ => read k)) s) =
+      get_payload ((bind (read k) (fun v => ret v)) s). 
+  Proof.
+    intros. apply extract_payload_read_read. apply read_and_read_lemma. auto.
+  Qed.
+
+  Theorem read_write :
+    forall (k : K) (v : V) (s : S),
+      well_formed s ->
+      get_payload ((bind (write k v) (fun _ => read k)) s) =
+      get_payload ((bind (write k v) (fun _ => ret (wrap v))) s).
+  Proof.
+    intros. rewrite read_and_write_compat_lemma_1; auto.
+    rewrite read_and_write_compat_lemma_2.
+    apply PathORAM_simulates_RAM. apply H.
+  Qed.
+
+  Theorem read_write_commute :
+    forall (k1 k2 : K) (v : V) f (s : S),
+      well_formed s ->
+      k1 <> k2 ->
+      get_payload (bind (read k1) (fun v' => bind (write k2 v) (fun _ => f v')) s) =
+      get_payload (bind (write k2 v) (fun _ => bind (read k1) f) s).
+  Proof.
+  Admitted.
+
+  Theorem read_commute :
+    forall (k1 k2 : K) f (s : S),
+      well_formed s ->
+      get_payload (bind (read k1) (fun v1 => bind (read k2) (fun v2 => f v1 v2)) s) =
+      get_payload (bind (read k2) (fun v2 => bind (read k1) (fun v1 => f v1 v2)) s).
+  Proof.
+  Admitted.
+
 End PathORAM.
+
